a non-det small-step semantics for interesting insns (ret/call/bop/mop/gep), proved   1) det small-step (dsInsn) is its instance   2) progress and preservation
Changed some definitions, s.t. the new semantics proofs can reuse
existing proofs amap.

An interesting case of the proofs is proving that a set of values is
inhabited, so a program is not stuck by accessing an empty set of values
in a well-formed program.



git-svn-id: https://webdav.seas.upenn.edu/svn/sol/vol@3029 eef5ea85-cc2e-0410-bd84-0fae1f012da8

src/ssa/genericvalues.v
@@ -231,8 +231,8 @@ match (intConsts2Nats TD cidxs) with
   end
 end.
 
-Definition mtrunc (TD:TargetData) (op:truncop) (t1:typ) (gv1:GenericValue) 
-  (t2:typ) : option GenericValue :=
+Definition mtrunc (TD:TargetData) (op:truncop) (t1:typ) (t2:typ) 
+  (gv1:GenericValue) : option GenericValue :=
 match GV2val TD gv1 with
 | Some (Vint wz1 i1) =>
     match (t1, t2) with
@@ -336,7 +336,7 @@ Definition mbitcast (t1:typ) (gv1:GenericValue)(t2:typ) : option GenericValue :=
 match (t1, t2) with
 | (typ_int sz1, typ_int sz2) => Some gv1
 | (typ_pointer _, typ_pointer _) => Some gv1
-| _ => None
+| _ => Some gundef
 end.
 
 Definition minttoptr (TD:TargetData) (M:mem) (gv1:GenericValue) 
@@ -384,23 +384,23 @@ Definition minttoptr (TD:TargetData) (M:mem) (gv1:GenericValue)
    to be undef, and integers from p2i to be undef, too.
    
 *)
-Definition mcast (TD:TargetData) (op:castop) (t1:typ) (gv1:GenericValue)
-  (t2:typ) : option GenericValue :=
+Definition mcast (TD:TargetData) (op:castop) (t1:typ) (t2:typ) (gv1:GenericValue)
+ : option GenericValue :=
 match op with
 | castop_inttoptr => 
   match (t1, t2) with
   | (typ_int sz1, typ_pointer _) => Some gundef
-  | _ => None
+  | _ => Some gundef
   end
 | castop_ptrtoint => 
   match (t1, t2) with
   | (typ_pointer _, typ_int sz2) => Some gundef
-  | _ => None
+  | _ => Some gundef
   end
 | castop_bitcase => mbitcast t1 gv1 t2 
 end.
 
-Definition mext (TD:TargetData) (op:extop) (t1:typ) (gv1:GenericValue) (t2:typ) 
+Definition mext (TD:TargetData) (op:extop) (t1:typ) (t2:typ) (gv1:GenericValue) 
   : option GenericValue :=
 match (t1, t2) with
 | (typ_int sz1, typ_int sz2) => 
@@ -639,7 +639,7 @@ match c with
 | const_truncop op c1 t2 =>
          match _const2GV TD gl c1 with
          | Some (gv1, t1) => 
-           match mtrunc TD op t1 gv1 t2 with
+           match mtrunc TD op t1 t2 gv1 with
            | Some gv2 => Some (gv2, t2)
            | _ => None
            end
@@ -648,7 +648,7 @@ match c with
 | const_extop op c1 t2 =>
          match _const2GV TD gl c1 with
          | Some (gv1, t1) => 
-           match mext TD op t1 gv1 t2 with
+           match mext TD op t1 t2 gv1 with
            | Some gv2 => Some (gv2, t2)
            | _ => None
            end
@@ -657,7 +657,7 @@ match c with
 | const_castop op c1 t2 =>
          match _const2GV TD gl c1 with
          | Some (gv1, t1) => 
-           match mcast TD op t1 gv1 t2 with
+           match mcast TD op t1 t2 gv1 with
            | Some gv2 => Some (gv2, t2)
            | _ => None
            end
@@ -908,7 +908,7 @@ end
 Definition TRUNC (TD:TargetData) (lc gl:GVMap) (op:truncop) (t1:typ) 
   (v1:value) (t2:typ) : option GenericValue :=
 match (getOperandValue TD v1 lc gl) with
-| (Some gv1) => mtrunc TD op t1 gv1 t2
+| (Some gv1) => mtrunc TD op t1 t2 gv1
 | _ => None
 end
 .
@@ -916,7 +916,7 @@ end
 Definition CAST (TD:TargetData) (lc gl:GVMap) (op:castop) (t1:typ) 
   (v1:value) (t2:typ) : option GenericValue:=
 match (getOperandValue TD v1 lc gl) with
-| (Some gv1) => mcast TD op t1 gv1 t2
+| (Some gv1) => mcast TD op t1 t2 gv1
 | _ => None
 end
 .
@@ -924,7 +924,7 @@ end
 Definition EXT (TD:TargetData) (lc gl:GVMap) (op:extop) (t1:typ) 
   (v1:value) (t2:typ) : option GenericValue :=
 match (getOperandValue TD v1 lc gl) with
-| (Some gv1) => mext TD op t1 gv1 t2
+| (Some gv1) => mext TD op t1 t2 gv1
 | _ => None
 end
 .
@@ -1024,13 +1024,13 @@ Lemma CAST_inversion : forall TD lc gl op t1 v1 t2 gv,
   CAST TD lc gl op t1 v1 t2 = Some gv ->
   exists gv1,
     getOperandValue TD v1 lc gl = Some gv1 /\
-    mcast TD op t1 gv1 t2 = Some gv.
+    mcast TD op t1 t2 gv1 = Some gv.
 Proof.
   intros TD lc gl op t1 v1 t2 gv HCAST.
   unfold CAST in HCAST.
   remember (getOperandValue TD v1 lc gl) as ogv1.
   destruct ogv1; try solve [inversion HCAST].
-    remember (mcast TD op t1 g t2) as R.
+    remember (mcast TD op t1 t2 g) as R.
     destruct R; inversion HCAST; subst.
       exists g. auto.
 Qed.
@@ -1039,13 +1039,13 @@ Lemma TRUNC_inversion : forall TD lc gl op t1 v1 t2 gv,
   TRUNC TD lc gl op t1 v1 t2 = Some gv ->
   exists gv1,
     getOperandValue TD v1 lc gl = Some gv1 /\
-    mtrunc TD op t1 gv1 t2 = Some gv.
+    mtrunc TD op t1 t2 gv1 = Some gv.
 Proof.
   intros TD lc gl op t1 v1 t2 gv HTRUNC.
   unfold TRUNC in HTRUNC.
   remember (getOperandValue TD v1 lc gl) as ogv1.
   destruct ogv1; try solve [inversion HTRUNC].
-    remember (mtrunc TD op t1 g t2) as R.
+    remember (mtrunc TD op t1 t2 g) as R.
     destruct R; inversion HTRUNC; subst.
       exists g. auto.
 Qed.
@@ -1054,13 +1054,13 @@ Lemma EXT_inversion : forall TD lc gl op t1 v1 t2 gv,
   EXT TD lc gl op t1 v1 t2 = Some gv ->
   exists gv1,
     getOperandValue TD v1 lc gl = Some gv1 /\
-    mext TD op t1 gv1 t2 = Some gv.
+    mext TD op t1 t2 gv1 = Some gv.
 Proof.
   intros TD lc gl op t1 v1 t2 gv HEXT.
   unfold EXT in HEXT.
   remember (getOperandValue TD v1 lc gl) as ogv1.
   destruct ogv1; try solve [inversion HEXT].
-    remember (mext TD op t1 g t2) as R.
+    remember (mext TD op t1 t2 g) as R.
     destruct R; inversion HEXT; subst.
       exists g. auto.
 Qed.
