src/ssa/ndopsem.v
@@ -1,0 +1,943 @@
+Add LoadPath "./ott".
+Add LoadPath "./monads".
+Add LoadPath "./compcert".
+Add LoadPath "../../../theory/metatheory_8.3".
+Require Import ssa_def.
+Require Import ssa_lib.
+Require Import List.
+Require Import Arith.
+Require Import tactics.
+Require Import monad.
+Require Import trace.
+Require Import Metatheory.
+Require Import genericvalues.
+Require Import alist.
+Require Import Values.
+Require Import Memory.
+Require Import Integers.
+Require Import Coqlib.
+Require Import targetdata.
+Require Import Ensembles.
+Require Import ssa_dynamic.
+
+Module NDopsem.
+
+Export LLVMsyntax.
+Export LLVMlib.
+Export LLVMgv.
+Export LLVMtd.
+
+Definition GVs := Ensemble GenericValue.
+Definition GVsMap := list (id * GVs).
+
+(**************************************)
+(** Execution contexts *)
+
+Record ExecutionContext : Type := mkEC {
+CurFunction : fdef;
+CurBB       : block;
+CurCmds     : cmds;                  (* cmds to run within CurBB *)
+Terminator  : terminator;
+Locals      : GVsMap;                (* LLVM values used in this invocation *)
+Allocas     : list mblock            (* Track memory allocated by alloca *)
+}.
+
+Definition ECStack := list ExecutionContext.
+
+(* FunTable maps function names to their addresses that are taken as function 
+   pointers. When we are calling a function via an id, we first search in Globals
+   via the value id to get its address, and then search in FunTable to get its
+   name, via the name, we search in CurProducts to get its definition.
+
+   We assume that there is an 'initFunTable' that returns function addresses to
+   initialize FunTable
+*)
+Record State : Type := mkState {
+CurSystem          : system;
+CurTargetData      : TargetData;
+CurProducts        : list product;
+ECS                : ECStack;
+Globals            : GVMap;
+FunTable           : GVMap;
+Mem                : mem
+}.
+
+Lemma singleton_inhabited : forall U (x:U), Inhabited U (Singleton U x).
+Proof.
+  intros. apply Inhabited_intro with (x:=x); auto using In_singleton.
+Qed.
+
+Lemma full_set_inhabited : Inhabited GenericValue (Full_set GenericValue).
+Proof.
+  intros. apply Inhabited_intro with (x:=nil); auto using Full_intro.
+Qed.
+
+Definition gv2gvs (gv:GenericValue) : GVs :=
+match gv with
+| (Vundef, _)::_ => Full_set _
+| _ => Singleton GenericValue gv
+end.
+
+Notation "$ gv $" := (gv2gvs gv) (at level 41).
+Notation "% ogv %" := (mmap GenericValue GVs gv2gvs ogv) (at level 41).
+Notation "gv @ gvs" := (Ensembles.In GenericValue gvs gv) 
+                         (at level 43, right associativity).
+
+Definition getOperandValue (TD:TargetData) (v:value) (locals:GVsMap) 
+  (globals:GVMap) : option GVs := 
+match v with
+| value_id id => lookupAL _ locals id 
+| value_const c => % (const2GV TD globals c) %
+end.
+
+Definition returnUpdateLocals (TD:TargetData) (c':cmd) (Result:value) 
+  (lc lc':GVsMap) (gl:GVMap) : option GVsMap :=
+  match (getOperandValue TD Result lc gl) with
+  | Some gr =>    
+      match (getCallerReturnID c') with
+      | Some id0 => Some (updateAddAL _ lc' id0 gr)
+      | None => Some lc'
+      end
+  | None => None
+  end.
+
+Fixpoint getIncomingValuesForBlockFromPHINodes (TD:TargetData)
+  (PNs:list phinode) (b:block) (globals:GVMap) (locals:GVsMap) : 
+  option (list (id*GVs)) :=
+match PNs with
+| nil => Some nil
+| (insn_phi id0 t vls)::PNs => 
+  match (getValueViaBlockFromPHINode (insn_phi id0 t vls) b) with
+  | None => None
+  | Some v => 
+      match (getOperandValue TD v locals globals, 
+             getIncomingValuesForBlockFromPHINodes TD PNs b globals locals)
+      with
+      | (Some gv1, Some idgvs) => Some ((id0,gv1)::idgvs)
+      | _ => None
+      end               
+  end
+end.
+
+Fixpoint updateValuesForNewBlock (ResultValues:list (id*GVs)) (locals:GVsMap) 
+  : GVsMap :=
+match ResultValues with
+| nil => locals
+| (id, v)::ResultValues' => 
+    updateAddAL _ (updateValuesForNewBlock ResultValues' locals) id v
+end.
+
+Definition switchToNewBasicBlock (TD:TargetData) (Dest:block) 
+  (PrevBB:block) (globals: GVMap) (locals:GVsMap): option GVsMap :=
+  let PNs := getPHINodesFromBlock Dest in
+  match getIncomingValuesForBlockFromPHINodes TD PNs PrevBB globals locals with
+  | Some ResultValues => Some (updateValuesForNewBlock ResultValues locals)
+  | None => None
+  end.
+
+Lemma gv_in_gv2gvs : forall gv, gv @ $ gv $.
+Proof.
+  intros.
+  destruct gv; simpl.
+    apply In_singleton; auto.
+    destruct p; simpl.
+    destruct v; simpl; auto using In_singleton.
+      apply Full_intro.
+Qed.
+
+Definition lift_op2 (f: GenericValue -> GenericValue -> option GenericValue)
+  gvs1 gvs2 : GVs :=
+  fun gv3 => exists gv1, exists gv2, exists gv3',
+    gv1 @ gvs1 /\ gv2 @ gvs2 /\ f gv1 gv2 = Some gv3' /\ (gv3 @ $ gv3' $).
+
+Definition BOP (TD:TargetData) (lc:GVsMap) (gl:GVMap) (op:bop) (bsz:sz) 
+  (v1 v2:value) : option GVs :=
+match (getOperandValue TD v1 lc gl, getOperandValue TD v2 lc gl) with
+| (Some gvs1, Some gvs2) => Some (lift_op2 (mbop TD op bsz) gvs1 gvs2)
+| _ => None
+end
+.
+
+Definition lift_op1 (f: GenericValue -> option GenericValue) gvs1 : GVs :=
+  fun gv2 => exists gv1, exists gv2', 
+    gv1 @ gvs1 /\ f gv1 = Some gv2' /\ (gv2 @ $ gv2' $).
+
+Definition CAST (TD:TargetData) (lc:GVsMap) (gl:GVMap) (op:castop) 
+  (t1:typ) (v1:value) (t2:typ) : option GVs:=
+match (getOperandValue TD v1 lc gl) with
+| (Some gvs1) => Some (lift_op1 (mcast TD op t1 t2) gvs1)
+| _ => None
+end
+.
+
+Fixpoint values2GVs (TD:TargetData) (lv:list_value) (locals:GVsMap) 
+  (globals:GVMap) : option (list GVs):=
+match lv with
+| Nil_list_value => Some nil
+| Cons_list_value v lv' => 
+  match (getOperandValue TD v locals globals) with
+  | Some GV => 
+    match (values2GVs TD lv' locals globals) with
+    | Some GVs => Some (GV::GVs)
+    | None => None
+    end
+  | None => None
+  end
+end.
+
+Fixpoint in_list_gvs (l1 : list GenericValue) (l2 : list GVs) :=
+match l1, l2 with
+| nil, nil => True
+| gv1::l1', gvs2::l2' => gv1 @ gvs2 /\ in_list_gvs l1' l2'
+| _, _ => False
+end.
+
+Notation "vidxs @@ vidxss" := (in_list_gvs vidxs vidxss) 
+  (at level 43, right associativity).
+
+Definition GEP (TD:TargetData) (t:typ) (mas:GVs) (vidxss:list GVs) 
+  (inbounds:bool) : option GVs :=
+  Some (fun gv => exists ma, exists vidxs, ma @ mas /\ vidxs @@ vidxss /\
+        LLVMgv.GEP TD t ma vidxs inbounds = Some gv).
+
+Fixpoint params2GVs (TD:TargetData) (lp:params) (locals:GVsMap) (globals:GVMap) :
+ option (list GVs) :=
+match lp with
+| nil => Some nil
+| (_, v)::lp' => 
+    match (getOperandValue TD v locals globals, 
+           params2GVs TD lp' locals globals) with
+    | (Some gv, Some gvs) => Some (gv::gvs)
+    | _ => None
+    end
+end.
+
+Fixpoint _initializeFrameValues (la:args) (lg:list GVs) (locals:GVsMap) 
+  : GVsMap :=
+match (la, lg) with
+| ((_, id)::la', g::lg') => 
+  updateAddAL _ (_initializeFrameValues la' lg' locals) id g
+| ((t, id)::la', nil) => 
+  (* FIXME: We should initalize them w.r.t their type size. *)
+  updateAddAL _ (_initializeFrameValues la' nil locals) id (Full_set _)
+| _ => locals
+end.
+
+Definition initLocals (la:args) (lg:list GVs): GVsMap := 
+_initializeFrameValues la lg nil.
+
+Definition lookupFdefViaPtr Ps fs fptr : option fdef :=
+  do fn <- LLVMopsem.lookupFdefViaGVFromFunTable fs fptr;
+     lookupFdefViaIDFromProducts Ps fn.
+
+Inductive sInsn : State -> State -> trace -> Prop :=
+| sReturn : forall S TD Ps F B rid RetTy Result lc gl fs
+                            F' B' c' cs' tmn' lc' EC
+                            Mem Mem' als als' lc'',   
+  Instruction.isCallInst c' = true ->
+  (* FIXME: we should get Result before free?! *)
+  free_allocas TD Mem als = Some Mem' ->
+  returnUpdateLocals TD c' Result lc lc' gl = Some lc'' ->
+  sInsn 
+    (mkState S TD Ps ((mkEC F B nil (insn_return rid RetTy Result) lc als)::
+                      (mkEC F' B' (c'::cs') tmn' lc' als')::EC) gl fs Mem)
+    (mkState S TD Ps ((mkEC F' B' cs' tmn' lc'' als')::EC) gl fs Mem')
+    trace_nil 
+
+| sReturnVoid : forall S TD Ps F B rid lc gl fs
+                            F' B' c' tmn' lc' EC
+                            cs' Mem Mem' als als',   
+  Instruction.isCallInst c' = true ->
+  free_allocas TD Mem als = Some Mem' ->
+  getCallerReturnID c' = None ->
+  sInsn 
+    (mkState S TD Ps ((mkEC F B nil (insn_return_void rid) lc als)::
+                      (mkEC F' B' (c'::cs') tmn' lc' als')::EC) gl fs Mem)
+    (mkState S TD Ps ((mkEC F' B' cs' tmn' lc' als')::EC) gl fs Mem')
+    trace_nil 
+
+| sBranch : forall S TD Ps F B lc gl fs bid Cond l1 l2 conds c
+                              l' ps' cs' tmn' lc' EC Mem als,   
+  getOperandValue TD Cond lc gl = Some conds ->
+  c @ conds ->
+  Some (block_intro l' ps' cs' tmn') = (if isGVZero TD c
+               then lookupBlockViaLabelFromFdef F l2
+               else lookupBlockViaLabelFromFdef F l1) ->
+  switchToNewBasicBlock TD (block_intro l' ps' cs' tmn') B gl lc = Some lc'->
+  sInsn 
+    (mkState S TD Ps ((mkEC F B nil (insn_br bid Cond l1 l2) lc als)::EC) 
+                       gl fs Mem)
+    (mkState S TD Ps ((mkEC F (block_intro l' ps' cs' tmn') cs' tmn' lc' als)
+                       ::EC) gl fs Mem)
+    trace_nil 
+
+| sBranch_uncond : forall S TD Ps F B lc gl fs bid l 
+                           l' ps' cs' tmn' lc' EC Mem als,   
+  Some (block_intro l' ps' cs' tmn') = (lookupBlockViaLabelFromFdef F l) ->
+  switchToNewBasicBlock TD (block_intro l' ps' cs' tmn') B gl lc = Some lc'->
+  sInsn 
+    (mkState S TD Ps ((mkEC F B nil (insn_br_uncond bid l) lc als)::EC) 
+                       gl fs Mem)
+    (mkState S TD Ps ((mkEC F (block_intro l' ps' cs' tmn') cs' tmn' lc' als)
+                       ::EC) gl fs Mem)
+    trace_nil 
+
+| sBop: forall S TD Ps F B lc gl fs id bop sz v1 v2 gvs3 EC cs tmn Mem als,
+  BOP TD lc gl bop sz v1 v2 = Some gvs3 ->
+  sInsn 
+    (mkState S TD Ps ((mkEC F B ((insn_bop id bop sz v1 v2)::cs) tmn lc als)
+                      ::EC) gl fs Mem) 
+    (mkState S TD Ps ((mkEC F B cs tmn (updateAddAL _ lc id gvs3) als)::EC) 
+                      gl fs Mem)
+    trace_nil 
+
+(*
+| sFBop: forall S TD Ps F B lc gl fs id fbop fp v1 v2 gv3 EC cs tmn Mem als,
+  FBOP TD lc gl fbop fp v1 v2 = Some gv3 ->
+  sInsn 
+    (mkState S TD Ps ((mkEC F B ((insn_fbop id fbop fp v1 v2)::cs) tmn lc 
+                       als)::EC) gl fs Mem) 
+    (mkState S TD Ps ((mkEC F B cs tmn (updateAddAL _ lc id gv3) als)::EC) 
+                      gl fs Mem)
+    trace_nil 
+
+| sExtractValue : forall S TD Ps F B lc gl fs id t v gv gv' idxs EC cs tmn 
+                          Mem als,
+  getOperandValue TD v lc gl = Some gv ->
+  extractGenericValue TD t gv idxs = Some gv' ->
+  sInsn 
+    (mkState S TD Ps ((mkEC F B ((insn_extractvalue id t v idxs)::cs) tmn lc
+                       als)::EC) gl fs Mem) 
+    (mkState S TD Ps ((mkEC F B cs tmn (updateAddAL _ lc id gv') als)::EC) 
+                       gl fs Mem)
+    trace_nil 
+
+| sInsertValue : forall S TD Ps F B lc gl fs id t v t' v' gv gv' gv'' idxs 
+                         EC cs tmn Mem als,
+  getOperandValue TD v lc gl = Some gv ->
+  getOperandValue TD v' lc gl = Some gv' ->
+  insertGenericValue TD t gv idxs t' gv' = Some gv'' ->
+  sInsn 
+    (mkState S TD Ps ((mkEC F B ((insn_insertvalue id t v t' v' idxs)::cs) tmn 
+                       lc als)::EC) gl fs Mem) 
+    (mkState S TD Ps ((mkEC F B cs tmn (updateAddAL _ lc id gv'') als)::EC) 
+                       gl fs Mem)
+    trace_nil 
+
+*)
+| sMalloc : forall S TD Ps F B lc gl fs id t v gns gn align EC cs tmn Mem als 
+                    Mem' tsz mb,
+  getTypeAllocSize TD t = Some tsz ->
+  getOperandValue TD v lc gl = Some gns ->
+  gn @ gns ->
+  malloc TD Mem tsz gn align = Some (Mem', mb) ->
+  sInsn 
+    (mkState S TD Ps ((mkEC F B ((insn_malloc id t v align)::cs) tmn lc als)
+                      ::EC) gl fs Mem) 
+    (mkState S TD Ps ((mkEC F B cs tmn 
+                        (updateAddAL _ lc id ($ (blk2GV TD mb) $)) 
+                      als)::EC) gl fs Mem')
+    trace_nil
+
+| sFree : forall S TD Ps F B lc gl fs fid t v EC cs tmn Mem als Mem' mptrs mptr,
+  getOperandValue TD v lc gl = Some mptrs ->
+  mptr @ mptrs ->
+  free TD Mem mptr = Some Mem'->
+  sInsn 
+    (mkState S TD Ps ((mkEC F B ((insn_free fid t v)::cs) tmn lc als)::EC) 
+                       gl fs Mem) 
+    (mkState S TD Ps ((mkEC F B cs tmn lc als)::EC) gl fs Mem')
+    trace_nil
+
+| sAlloca : forall S TD Ps F B lc gl fs id t v gns gn align EC cs tmn Mem als 
+                    Mem' tsz mb,
+  getTypeAllocSize TD t = Some tsz ->
+  getOperandValue TD v lc gl = Some gns ->
+  gn @ gns ->
+  malloc TD Mem tsz gn align = Some (Mem', mb) ->
+  sInsn 
+    (mkState S TD Ps ((mkEC F B ((insn_alloca id t v align)::cs) tmn lc als)
+                      ::EC) gl fs Mem) 
+    (mkState S TD Ps ((mkEC F B cs tmn 
+                        (updateAddAL _ lc id ($ (blk2GV TD mb) $)) 
+                      (mb::als))::EC) gl fs Mem')
+    trace_nil
+
+| sLoad : forall S TD Ps F B lc gl fs id t align v EC cs tmn Mem als mps mp gv,
+  getOperandValue TD v lc gl = Some mps ->
+  mp @ mps ->
+  mload TD Mem mp t align = Some gv ->
+  sInsn 
+    (mkState S TD Ps ((mkEC F B ((insn_load id t v align)::cs) tmn lc als)::
+                       EC) gl fs Mem) 
+    (mkState S TD Ps ((mkEC F B cs tmn (updateAddAL _ lc id ($ gv $)) als)::EC) 
+                       gl fs Mem)
+    trace_nil
+
+| sStore : forall S TD Ps F B lc gl fs sid t align v1 v2 EC cs tmn Mem als 
+                   mp2 gv1 Mem' gvs1 mps2,
+  getOperandValue TD v1 lc gl = Some gvs1 ->
+  getOperandValue TD v2 lc gl = Some mps2 ->
+  gv1 @ gvs1 -> mp2 @ mps2 ->
+  mstore TD Mem mp2 t gv1 align = Some Mem' ->
+  sInsn 
+    (mkState S TD Ps ((mkEC F B ((insn_store sid t v1 v2 align)::cs) tmn lc
+                       als)::EC) gl fs Mem) 
+    (mkState S TD Ps ((mkEC F B cs tmn lc als)::EC) gl fs Mem')
+    trace_nil
+
+| sGEP : forall S TD Ps F B lc gl fs id inbounds t v idxs vidxs EC mp mp' 
+                 cs tmn Mem als,
+  getOperandValue TD v lc gl = Some mp ->
+  values2GVs TD idxs lc gl = Some vidxs ->
+  GEP TD t mp vidxs inbounds = Some mp' ->
+  sInsn 
+    (mkState S TD Ps ((mkEC F B ((insn_gep id inbounds t v idxs)::cs) tmn lc
+                       als)::EC) gl fs Mem) 
+    (mkState S TD Ps ((mkEC F B cs tmn (updateAddAL _ lc id mp') als)::EC) 
+                       gl fs Mem)
+    trace_nil 
+(*
+| sTrunc : forall S TD Ps F B lc gl fs id truncop t1 v1 t2 gv2 EC cs tmn 
+                   Mem als,
+  TRUNC TD lc gl truncop t1 v1 t2 = Some gv2 ->
+  sInsn 
+    (mkState S TD Ps ((mkEC F B ((insn_trunc id truncop t1 v1 t2)::cs) tmn lc 
+                       als)::EC) gl fs Mem) 
+    (mkState S TD Ps ((mkEC F B cs tmn (updateAddAL _ lc id gv2) als)::EC) 
+                       gl fs Mem)
+    trace_nil
+
+| sExt : forall S TD Ps F B lc gl fs id extop t1 v1 t2 gv2 EC cs tmn Mem 
+                 als,
+  EXT TD lc gl extop t1 v1 t2 = Some gv2 ->
+  sInsn 
+    (mkState S TD Ps ((mkEC F B ((insn_ext id extop t1 v1 t2)::cs) tmn lc 
+                       als)::EC) gl fs Mem) 
+    (mkState S TD Ps ((mkEC F B cs tmn (updateAddAL _ lc id gv2) als)::EC) 
+                       gl fs Mem)
+    trace_nil
+*)
+| sCast : forall S TD Ps F B lc gl fs id castop t1 v1 t2 gv2 EC cs tmn Mem 
+                  als,
+  CAST TD lc gl castop t1 v1 t2 = Some gv2 ->
+  sInsn 
+    (mkState S TD Ps ((mkEC F B ((insn_cast id castop t1 v1 t2)::cs) tmn lc 
+                      als)::EC) gl fs Mem) 
+    (mkState S TD Ps ((mkEC F B cs tmn (updateAddAL _ lc id gv2) als)::EC) 
+                      gl fs Mem)
+    trace_nil
+(*
+| sIcmp : forall S TD Ps F B lc gl fs id cond t v1 v2 gv3 EC cs tmn Mem als,
+  ICMP TD lc gl cond t v1 v2 = Some gv3 ->
+  sInsn 
+    (mkState S TD Ps ((mkEC F B ((insn_icmp id cond t v1 v2)::cs) tmn lc als)
+                      ::EC) gl fs Mem) 
+    (mkState S TD Ps ((mkEC F B cs tmn (updateAddAL _ lc id gv3) als)::EC) 
+                       gl fs Mem)
+    trace_nil
+
+| sFcmp : forall S TD Ps F B lc gl fs id fcond fp v1 v2 gv3 EC cs tmn Mem 
+                  als,
+  FCMP TD lc gl fcond fp v1 v2 = Some gv3 ->
+  sInsn 
+    (mkState S TD Ps ((mkEC F B ((insn_fcmp id fcond fp v1 v2)::cs) tmn lc 
+                       als)::EC) gl fs Mem) 
+    (mkState S TD Ps ((mkEC F B cs tmn (updateAddAL _ lc id gv3) als)::EC) 
+                       gl fs Mem)
+    trace_nil
+
+| sSelect : forall S TD Ps F B lc gl fs id v0 t v1 v2 c EC cs tmn Mem als 
+                    gv1 gv2,
+  getOperandValue TD v0 lc gl = Some c ->
+  getOperandValue TD v1 lc gl = Some gv1 ->
+  getOperandValue TD v2 lc gl = Some gv2 ->
+  sInsn 
+    (mkState S TD Ps ((mkEC F B ((insn_select id v0 t v1 v2)::cs) tmn lc als)
+                      ::EC) gl fs Mem) 
+    (mkState S TD Ps ((mkEC F B cs tmn (if isGVZero TD c 
+                                        then updateAddAL _ lc id gv2 
+                                        else updateAddAL _ lc id gv1) als)
+                      ::EC) gl fs Mem)
+    trace_nil
+*)
+| sCall : forall S TD Ps F B lc gl fs rid noret ca fid fv lp cs tmn fptrs fptr
+                       l' ps' cs' tmn' EC rt la va lb Mem als ft fa gvs,
+  (* only look up the current module for the time being, 
+     do not support linkage. *)
+  getOperandValue TD fv lc gl = Some fptrs -> 
+  fptr @ fptrs -> 
+  lookupFdefViaPtr Ps fs fptr = 
+    Some (fdef_intro (fheader_intro fa rt fid la va) lb) ->
+  getEntryBlock (fdef_intro (fheader_intro fa rt fid la va) lb) = 
+    Some (block_intro l' ps' cs' tmn') ->
+  params2GVs TD lp lc gl = Some gvs ->
+  sInsn 
+    (mkState S TD Ps ((mkEC F B ((insn_call rid noret ca ft fv lp)::cs) tmn 
+                       lc als)::EC) gl fs Mem)
+    (mkState S TD Ps ((mkEC (fdef_intro (fheader_intro fa rt fid la va) lb) 
+                       (block_intro l' ps' cs' tmn') cs' tmn' 
+                       (initLocals la gvs) 
+                       nil)::
+                      (mkEC F B ((insn_call rid noret ca ft fv lp)::cs) tmn 
+                       lc als)::EC) gl fs Mem)
+    trace_nil 
+(*
+| sExCall : forall S TD Ps F B lc gl fs rid noret ca fid fv lp cs tmn EC 
+                    rt la Mem als oresult Mem' lc' va ft fa gvs,
+  (* only look up the current module for the time being, 
+     do not support linkage. 
+     FIXME: should add excall to trace
+  *)
+  lookupExFdecViaGV TD Ps gl lc fs fv = 
+    Some (fdec_intro (fheader_intro fa rt fid la va)) ->
+  params2GVs TD lp lc gl = Some gvs ->
+  callExternalFunction Mem fid gvs = Some (oresult, Mem') ->
+  exCallUpdateLocals noret rid oresult lc = Some lc' ->
+  sInsn 
+    (mkState S TD Ps ((mkEC F B ((insn_call rid noret ca ft fv lp)::cs) tmn 
+                       lc als)::EC) gl fs Mem)
+    (mkState S TD Ps ((mkEC F B cs tmn lc' als)::EC) gl fs Mem')
+    trace_nil 
+*).
+
+Hint Constructors sInsn.
+
+Definition s_genInitState (S:system) (main:id) (Args:list GVs) (initmem:mem) 
+  : option State :=
+match (lookupFdefViaIDFromSystem S main) with
+| None => None
+| Some CurFunction =>
+  match (getParentOfFdefFromSystem CurFunction S) with
+  | None => None
+  | Some (module_intro CurLayouts CurNamedts CurProducts) =>
+    let initargetdata := 
+      LLVMopsem.initTargetData CurLayouts CurNamedts initmem in 
+    match (LLVMopsem.genGlobalAndInitMem initargetdata CurProducts nil nil 
+      initmem) with
+    | None => None
+    | Some (initGlobal, initFunTable, initMem) =>
+      match (getEntryBlock CurFunction) with
+      | None => None
+      | Some (block_intro l ps cs tmn) => 
+          match CurFunction with 
+          | fdef_intro (fheader_intro _ rt _ la _) _ =>
+            let Values := initLocals la Args in
+              Some
+              (mkState
+                S
+                initargetdata
+                CurProducts
+                ((mkEC
+                  CurFunction 
+                  (block_intro l ps cs tmn) 
+                  cs
+                  tmn
+                  Values 
+                  nil
+                )::nil)
+                initGlobal
+                initFunTable
+                initMem
+            )          
+        end
+      end
+    end
+  end
+end.
+
+Definition s_isFinialState (state:State) : bool :=
+match state with
+| (mkState _ _ _ ((mkEC _ _ nil (insn_return_void _) _ _)::nil) _ _ _) => true
+| (mkState _ _ _ ((mkEC _ _ nil (insn_return _ _ _) _ _)::nil) _ _ _) => true 
+| _ => false
+end.
+
+Inductive sop_star : State -> State -> trace -> Prop :=
+| sop_star_nil : forall state, sop_star state state trace_nil
+| sop_star_cons : forall state1 state2 state3 tr1 tr2,
+    sInsn state1 state2 tr1 ->
+    sop_star state2 state3 tr2 ->
+    sop_star state1 state3 (trace_app tr1 tr2)
+.
+
+Inductive sop_plus : State -> State -> trace -> Prop :=
+| sop_plus_cons : forall state1 state2 state3 tr1 tr2,
+    sInsn state1 state2 tr1 ->
+    sop_star state2 state3 tr2 ->
+    sop_plus state1 state3 (trace_app tr1 tr2)
+.
+
+CoInductive sop_diverges : State -> Trace -> Prop :=
+| sop_diverges_intro : forall state1 state2 tr1 tr2,
+    sop_plus state1 state2 tr1 ->
+    sop_diverges state2 tr2 ->
+    sop_diverges state1 (Trace_app tr1 tr2)
+.
+
+Inductive s_converges : system -> id -> list GVs -> State -> Prop :=
+| s_converges_intro : forall (s:system) (main:id) (VarArgs:list GVs) 
+                              (IS FS:State) tr,
+  s_genInitState s main VarArgs Mem.empty = Some IS ->
+  sop_star IS FS tr ->
+  s_isFinialState FS ->
+  s_converges s main VarArgs FS
+.
+
+Inductive s_diverges : system -> id -> list GVs -> Trace -> Prop :=
+| s_diverges_intro : forall (s:system) (main:id) (VarArgs:list GVs) 
+                             (IS:State) tr,
+  s_genInitState s main VarArgs Mem.empty = Some IS ->
+  sop_diverges IS tr ->
+  s_diverges s main VarArgs tr
+.
+
+Inductive s_goeswrong : system -> id -> list GVs -> State -> Prop :=
+| s_goeswrong_intro : forall (s:system) (main:id) (VarArgs:list GVs) 
+                              (IS FS:State) tr,
+  s_genInitState s main VarArgs Mem.empty = Some IS ->
+  sop_star IS FS tr ->
+  ~ s_isFinialState FS ->
+  s_goeswrong s main VarArgs FS
+.
+
+Fixpoint instantiate_locals (lc1 : GVMap) (lc2 : GVsMap) : Prop :=
+match lc1, lc2 with
+| nil, nil => True
+| (id1,gv1)::lc1', (id2,gvs2)::lc2' => 
+    id1=id2 /\ gv1 @ gvs2 /\ instantiate_locals lc1' lc2'
+| _, _ => False
+end.
+
+Definition instantiate_EC (ec1 : LLVMopsem.ExecutionContext) 
+  (ec2 : ExecutionContext) : Prop :=
+match ec1, ec2 with
+| LLVMopsem.mkEC f1 b1 cs1 tmn1 lc1 als1, mkEC f2 b2 cs2 tmn2 lc2 als2 =>
+    f1 = f2 /\ b1 = b2 /\ cs1 = cs2 /\ tmn1 = tmn2 /\
+    instantiate_locals lc1 lc2 /\ als1 = als2
+end.
+
+Fixpoint instantiate_ECs (ecs1 : LLVMopsem.ECStack) (ecs2 : ECStack) : Prop :=
+match ecs1, ecs2 with
+| nil, nil => True
+| ec1::ecs1', ec2::ecs2' => instantiate_EC ec1 ec2 /\ instantiate_ECs ecs1' ecs2'
+| _, _ => False
+end.
+
+Definition instantiate_State (st1 : LLVMopsem.State) (st2 : State) : Prop :=
+match st1, st2 with
+| LLVMopsem.mkState s1 td1 ps1 ecs1 gl1 fs1 M1,
+  mkState s2 td2 ps2 ecs2 gl2 fs2 M2 =>
+    s1 = s2 /\ td1 = td2 /\ ps1 = ps2 /\ instantiate_ECs ecs1 ecs2 /\ gl1 = gl2
+    /\ fs1 = fs2 /\ M1 = M2
+end.
+
+Export LLVMopsem.
+
+Ltac simpl_nd_llvmds :=
+  match goal with
+  | [Hsim : instantiate_State {| ECS := _::_::_ |} ?st2 |- _ ] =>
+     destruct st2 as [S' TD' Ps' ECs' gl' fs' M'];
+     destruct Hsim as [eq1 [eq2 [eq3 [Hsim [eq4 [eq5 eq6]]]]]]; subst;
+     destruct ECs' as [|[f1' b1' cs1' tmn1' lc1' als1'] ECs']; 
+       try solve [inversion Hsim];
+     simpl in Hsim; destruct Hsim as [Hsim1 Hsim2];
+     destruct ECs' as [|[f2' b2' cs2' tmn2' lc2' als2'] ECs'];
+       try solve [inversion Hsim2];
+     destruct Hsim2 as [Hsim2 Hsim3];
+     destruct Hsim1 as [J1 [J2 [J3 [J4 [Hsim1 J6]]]]]; subst;
+     destruct Hsim2 as [J1 [J2 [J3 [J4 [Hsim2 J6]]]]]; subst
+  | [Hsim : instantiate_State {| ECS := _::_|} ?st2 |- _ ] =>
+     destruct st2 as [S' TD' Ps' ECs' gl' fs' M'];
+     destruct Hsim as [eq1 [eq2 [eq3 [Hsim [eq4 [eq5 eq6]]]]]]; subst;
+     destruct ECs' as [|[f1' b1' cs1' tmn1' lc1' als1'] ECs']; 
+       try solve [inversion Hsim];
+     simpl in Hsim; destruct Hsim as [Hsim1 Hsim2];
+     destruct Hsim1 as [J1 [J2 [J3 [J4 [Hsim1 J6]]]]]; subst
+  end.
+
+Lemma instantiate_locals__lookup : forall lc1 lc2 id1 gv1,
+  instantiate_locals lc1 lc2 -> 
+  lookupAL _ lc1 id1 = Some gv1 ->
+  exists gvs2, lookupAL _ lc2 id1 = Some gvs2 /\ gv1 @ gvs2.
+Proof.
+  induction lc1; destruct lc2; simpl; intros id1 gv1 Hinst Hlk.  
+    inv Hlk.
+    inv Hinst.
+    destruct a. inv Hinst.     
+
+    destruct a. destruct p.
+    destruct Hinst as [J1 [J2 J3]]; subst.
+    destruct (id1 == i1); subst; eauto.
+      inv Hlk. eauto.
+Qed.
+
+Lemma instantiate_locals__getOperandValue : forall TD v lc1 lc2 gl gv1,
+  instantiate_locals lc1 lc2 -> 
+  getOperandValue TD v lc1 gl = Some gv1 ->
+  exists gvs2, NDopsem.getOperandValue TD v lc2 gl = Some gvs2 /\
+    gv1 @ gvs2.
+Proof.
+  intros.
+  destruct v; simpl in *.
+    eapply instantiate_locals__lookup; eauto.
+    exists ($ gv1 $). unfold mmap. rewrite H0. simpl. 
+    auto using gv_in_gv2gvs.
+Qed.
+
+Lemma instantiate_locals__returnUpdateLocals : forall TD lc1 lc2 lc1' lc2' Result
+    gl lc1'' c,
+  instantiate_locals lc1 lc2 -> 
+  instantiate_locals lc1' lc2' -> 
+  returnUpdateLocals TD c Result lc1 lc1' gl = ret lc1'' ->
+  exists lc2'', 
+    NDopsem.returnUpdateLocals TD c Result lc2 lc2' gl = ret lc2'' /\
+    instantiate_locals lc1'' lc2''. 
+Proof.
+  intros.
+  unfold returnUpdateLocals in H1.
+
+Admitted.    
+
+Lemma instantiate_locals__switchToNewBasicBlock : forall TD lc1 lc2 gl lc1' b b',
+  instantiate_locals lc1 lc2 -> 
+  switchToNewBasicBlock TD b' b gl lc1 = Some lc1' ->
+  exists lc2', NDopsem.switchToNewBasicBlock TD b' b gl lc2 = Some lc2' /\
+    instantiate_locals lc1' lc2'. 
+Admitted.
+
+Lemma in_lift_op2 : forall f x y z xs ys,
+  f x y = Some z ->
+  x @ xs ->
+  y @ ys ->
+  z @ lift_op2 f xs ys.
+Proof.
+  intros. unfold lift_op2. 
+  unfold Ensembles.In.
+  exists x. exists y. exists z. rewrite H. 
+  repeat (split; auto).
+    apply gv_in_gv2gvs.
+Qed.
+
+Lemma instantiate_locals__BOP : forall TD lc1 lc2 gl v1 v2 gv3 bop sz,
+  instantiate_locals lc1 lc2 -> 
+  BOP TD lc1 gl bop sz v1 v2 = Some gv3 ->
+  exists gvs3', NDopsem.BOP TD lc2 gl bop sz v1 v2 = Some gvs3' /\
+    gv3 @ gvs3'.
+Proof.
+  intros.
+  apply BOP_inversion in H0.
+  destruct H0 as [gv1 [gv2 [J1 [J2 J3]]]].
+  eapply instantiate_locals__getOperandValue in J1; eauto.
+  destruct J1 as [gvs1 [H1 H2]].
+  eapply instantiate_locals__getOperandValue in J2; eauto.
+  destruct J2 as [gvs2 [H3 H4]].
+  unfold NDopsem.BOP.
+  rewrite H1. rewrite H3.
+  exists (lift_op2 (mbop TD bop0 sz0) gvs1 gvs2).
+  split; eauto using in_lift_op2.
+Qed.
+  
+Lemma instantiate_locals__updateAddAL : forall lc1 lc2 id0 gv3 gvs3',
+  instantiate_locals lc1 lc2 -> 
+  gv3 @ gvs3' ->
+  instantiate_locals (updateAddAL GenericValue lc1 id0 gv3)
+    (updateAddAL GVs lc2 id0 gvs3').
+Admitted.
+
+Lemma instantiate_locals__values2GVs : forall TD lc1 lc2 gl vidxs idxs,
+  instantiate_locals lc1 lc2 -> 
+  values2GVs TD idxs lc1 gl = Some vidxs ->
+  exists vidxss, NDopsem.values2GVs TD idxs lc2 gl = Some vidxss /\
+    vidxs @@ vidxss.
+Admitted.
+
+Lemma instantiate_locals__GEP : forall TD t mp1 mp1' vidxs vidxss inbounds mps2,
+  vidxs @@ vidxss ->
+  mp1 @ mps2 ->
+  GEP TD t mp1 vidxs inbounds = Some mp1' ->
+  exists mps2', NDopsem.GEP TD t mps2 vidxss inbounds = Some mps2' /\ 
+    mp1' @ mps2'.
+Admitted.
+
+Lemma instantiate_locals__CAST : forall TD lc1 lc2 gl t1 v1 t2 gv2 castop0,
+  instantiate_locals lc1 lc2 -> 
+  CAST TD lc1 gl castop0 t1 v1 t2 = Some gv2 ->
+  exists gvs2', NDopsem.CAST TD lc2 gl castop0 t1 v1 t2 = Some gvs2' 
+    /\ gv2 @ gvs2'.
+Admitted.
+
+Lemma lookupFdefViaGV_inversion : forall TD Ps gl lc fs fv f,
+  lookupFdefViaGV TD Ps gl lc fs fv = Some f ->
+  exists fptr, exists fn,
+    getOperandValue TD fv lc gl = Some fptr /\
+    lookupFdefViaGVFromFunTable fs fptr = Some fn /\
+    lookupFdefViaIDFromProducts Ps fn = Some f.
+Admitted.
+
+Lemma instantiate_locals__params2GVs : forall TD lc1 lc2 gl lp gvs1,
+  instantiate_locals lc1 lc2 ->
+  params2GVs TD lp lc1 gl = Some gvs1 ->
+  exists gvss2, NDopsem.params2GVs TD lp lc2 gl = Some gvss2 /\
+    gvs1 @@ gvss2.
+Admitted.
+
+Lemma instantiate_locals__initLocals : forall la gvs1 gvss2,
+  gvs1 @@ gvss2 ->
+  instantiate_locals (initLocals la gvs1) (NDopsem.initLocals la gvss2).
+Admitted.
+
+Lemma test : forall st1 st2 st1' tr,
+  instantiate_State st1 st2 ->
+  LLVMopsem.dsInsn st1 st1' tr ->
+  exists st2', sInsn st2 st2' tr /\ instantiate_State st1' st2'.
+Proof.
+  intros st1 st2 st1' tr Hsim Hop.  
+  (dsInsn_cases (induction Hop) Case).
+Case "dsReturn". simpl_nd_llvmds. 
+  eapply instantiate_locals__returnUpdateLocals in H1; eauto.
+  destruct H1 as [lc2'' [H1 H2]].
+  exists (NDopsem.mkState S' TD' Ps' 
+    ((NDopsem.mkEC f2' b2' cs' tmn2' lc2'' als2')::ECs') gl' fs' Mem').
+  split; eauto.
+    repeat (split; auto).
+Case "dsReturnVoid". simpl_nd_llvmds. 
+  exists (NDopsem.mkState S' TD' Ps' 
+    ((NDopsem.mkEC f2' b2' cs' tmn2' lc2' als2')::ECs') gl' fs' Mem').
+  split; eauto.
+    repeat (split; auto).
+Case "dsBranch". simpl_nd_llvmds. 
+  eapply instantiate_locals__switchToNewBasicBlock in H1; eauto.
+  eapply instantiate_locals__getOperandValue in H; eauto.
+  destruct H as [gvs2 [J1 J2]].
+  destruct H1 as [lc2' [J3 J4]].
+  exists (NDopsem.mkState S' TD' Ps' 
+    ((NDopsem.mkEC f1' (block_intro l' ps' cs' tmn') cs' tmn' lc2' als1')
+      ::ECs') gl' fs' M').
+  split; eauto.
+    repeat (split; auto).
+Case "dsBranch_uncond". simpl_nd_llvmds. 
+  eapply instantiate_locals__switchToNewBasicBlock in H0; eauto.
+  destruct H0 as [lc2' [J1 J2]].
+  exists (NDopsem.mkState S' TD' Ps' 
+    ((NDopsem.mkEC f1' (block_intro l' ps' cs' tmn') cs' tmn' lc2' als1')
+      ::ECs') gl' fs' M').
+  split; eauto.
+    repeat (split; auto).
+Case "dsBop". simpl_nd_llvmds. 
+  eapply instantiate_locals__BOP in H; eauto.
+  destruct H as [gvs3' [J1 J2]].
+  exists (NDopsem.mkState S' TD' Ps' 
+    ((NDopsem.mkEC f1' b1' cs tmn1' (updateAddAL _ lc1' id0 gvs3') als1')
+      ::ECs') gl' fs' M').
+  split; eauto.
+    repeat (split; auto using instantiate_locals__updateAddAL).
+Case "dsFBop". admit.
+Case "dsExtractValue". admit.
+Case "dsInsertValue". admit.
+Case "dsMalloc". simpl_nd_llvmds. 
+  eapply instantiate_locals__getOperandValue in H0; eauto.
+  destruct H0 as [gns [J1 J2]].
+  exists (NDopsem.mkState S' TD' Ps' 
+    ((NDopsem.mkEC f1' b1' cs tmn1' 
+      (updateAddAL _ lc1' id0 ($ (blk2GV TD' mb) $)) 
+    als1')::ECs') gl' fs' Mem').
+  split; eauto.
+    repeat (split; auto).
+      apply instantiate_locals__updateAddAL; auto.
+      unfold blk2GV, ptr2GV, val2GV.
+      apply gv_in_gv2gvs.
+Case "dsFree". simpl_nd_llvmds. 
+  eapply instantiate_locals__getOperandValue in H; eauto.
+  destruct H as [gvs [J1 J2]].
+  exists (NDopsem.mkState S' TD' Ps' 
+    ((NDopsem.mkEC f1' b1' cs tmn1' lc1'
+    als1')::ECs') gl' fs' Mem').
+  split; eauto.
+    repeat (split; auto).
+Case "dsAlloca". simpl_nd_llvmds. 
+  eapply instantiate_locals__getOperandValue in H0; eauto.
+  destruct H0 as [gns [J1 J2]].
+  exists (NDopsem.mkState S' TD' Ps' 
+    ((NDopsem.mkEC f1' b1' cs tmn1' 
+      (updateAddAL _ lc1' id0 ($ (blk2GV TD' mb) $)) 
+    (mb::als1'))::ECs') gl' fs' Mem').
+  split; eauto.
+    repeat (split; auto).
+      apply instantiate_locals__updateAddAL; auto.
+      unfold blk2GV, ptr2GV, val2GV.
+      apply gv_in_gv2gvs.
+Case "dsLoad". simpl_nd_llvmds. 
+  eapply instantiate_locals__getOperandValue in H; eauto.
+  destruct H as [gvs2 [J1 J2]].
+  exists (NDopsem.mkState S' TD' Ps' 
+    ((NDopsem.mkEC f1' b1' cs tmn1' (updateAddAL _ lc1' id0 ($ gv $))
+    als1')::ECs') gl' fs' M').
+  split; eauto.
+    repeat (split; auto using instantiate_locals__updateAddAL, gv_in_gv2gvs).
+Case "dsStore". simpl_nd_llvmds. 
+  eapply instantiate_locals__getOperandValue in H; eauto.
+  destruct H as [gvs2 [J1 J2]].
+  eapply instantiate_locals__getOperandValue in H0; eauto.
+  destruct H0 as [mps2 [J3 J4]].
+  exists (NDopsem.mkState S' TD' Ps' 
+    ((NDopsem.mkEC f1' b1' cs tmn1' lc1' als1')::ECs') gl' fs' Mem').
+  split; eauto.
+    repeat (split; auto).
+Case "dsGEP". simpl_nd_llvmds. 
+  eapply instantiate_locals__getOperandValue in H; eauto.
+  destruct H as [mps [J1 J2]].
+  eapply instantiate_locals__values2GVs in H0; eauto.
+  destruct H0 as [vidxss [J3 J4]].
+  eapply instantiate_locals__GEP in H1; eauto.
+  destruct H1 as [mps2' [J5 J6]].
+  exists (NDopsem.mkState S' TD' Ps' 
+    ((NDopsem.mkEC f1' b1' cs tmn1' (updateAddAL _ lc1' id0 mps2') als1')
+      ::ECs') gl' fs' M').
+  split; eauto.
+    repeat (split; auto using instantiate_locals__updateAddAL).
+Case "dsTrunc". admit.
+Case "dsExt". admit.
+Case "dsCast". simpl_nd_llvmds. 
+  eapply instantiate_locals__CAST in H; eauto.
+  destruct H as [gvs2' [J1 J2]].
+  exists (NDopsem.mkState S' TD' Ps' 
+    ((NDopsem.mkEC f1' b1' cs tmn1' (updateAddAL _ lc1' id0 gvs2') als1')
+      ::ECs') gl' fs' M').
+  split; eauto.
+    repeat (split; auto using instantiate_locals__updateAddAL).
+Case "dsIcmp". admit.
+Case "dsFcmp". admit.
+Case "dsSelect". admit.
+Case "dsCall". simpl_nd_llvmds. 
+  apply lookupFdefViaGV_inversion in H.
+  destruct H as [fptr [fn [J1 [J2 J3]]]].
+  eapply instantiate_locals__getOperandValue in J1; eauto.
+  destruct J1 as [gvs2 [J11 J12]].
+  eapply instantiate_locals__params2GVs in H1; eauto.
+  destruct H1 as [gvss2 [H11 H12]].
+  exists (NDopsem.mkState S' TD' Ps' 
+    ((NDopsem.mkEC (fdef_intro (fheader_intro fa rt fid la va) lb) 
+                       (block_intro l' ps' cs' tmn') cs' tmn' 
+                       (NDopsem.initLocals la gvss2) 
+                       nil)::
+     (NDopsem.mkEC f1' b1' (insn_call rid noret0 ca ft fv lp :: cs) tmn1' 
+      lc1' als1') ::ECs') gl' fs' M').
+  split.
+    eapply sCall; eauto.
+      unfold lookupFdefViaPtr. 
+      rewrite J2. simpl. rewrite J3. auto.
+    repeat (split; auto using instantiate_locals__initLocals).
+Case "dsExCall". admit.
+Qed.
+
+End NDopsem.
+
+
+(*****************************)
+(*
+*** Local Variables: ***
+*** coq-prog-name: "coqtop" ***
+*** coq-prog-args: ("-emacs-U" "-I" "~/SVN/sol/vol/src/ssa/monads" "-I" "~/SVN/sol/vol/src/ssa/ott" "-I" "~/SVN/sol/vol/src/ssa/compcert" "-I" "~/SVN/sol/theory/metatheory_8.3") ***
+*** End: ***
+ *)
