src/ssa/ndopsem_pp.v
@@ -1,0 +1,3151 @@
+Add LoadPath "./ott".
+Add LoadPath "./monads".
+Add LoadPath "./compcert".
+Add LoadPath "../../../theory/metatheory_8.3".
+Require Import ssa_def.
+Require Import ssa_lib.
+Require Import List.
+Require Import Arith.
+Require Import tactics.
+Require Import monad.
+Require Import trace.
+Require Import Metatheory.
+Require Import genericvalues.
+Require Import alist.
+Require Import Values.
+Require Import Memory.
+Require Import Integers.
+Require Import Coqlib.
+Require Import targetdata.
+Require Import Maps.
+Require Import Lattice.
+Require Import Iteration.
+Require Import Kildall.
+Require Import ssa_static.
+Require Import ssa_dynamic.
+Require Import ssa_props.
+Require Import ssa_analysis.
+Require Import ssa_wf.
+Require Import ndopsem.
+
+Export LLVMwf.
+Export AtomSet.
+
+(***************************)
+(* domination prop *)
+
+Export LLVMgv.
+Export NDopsem.
+
+Inductive wf_GVs : GVs -> typ -> Prop :=
+| wf_GVs_intro : forall gvs t, Ensembles.Inhabited _ gvs -> wf_GVs gvs t.
+
+Hint Constructors wf_GVs.
+
+Inductive wf_defs (f:fdef) (lc:GVsMap) : list atom -> Prop :=
+| wf_defs_nil : wf_defs f lc nil
+| wf_defs_cons : forall id1 t1 gvs1 defs',
+    lookupTypViaIDFromFdef f id1 = Some t1 ->
+    lookupAL _ lc id1 = Some gvs1 -> 
+    wf_GVs gvs1 t1 ->
+    wf_defs f lc defs' ->
+    wf_defs f lc (id1::defs').
+
+Lemma wf_defs_elim : forall ids1 F lc,
+  wf_defs F lc ids1 ->
+  forall id1, In id1 ids1 ->
+  exists t1, exists gvs1,
+    lookupTypViaIDFromFdef F id1 = Some t1 /\
+    lookupAL _ lc id1 = Some gvs1 /\
+    wf_GVs gvs1 t1.
+Proof.
+  induction ids1; intros; simpl in H0; inv H0.  
+    inv H.
+    exists t1. exists gvs1. split; auto.
+
+    inv H.
+    eapply IHids1 in H6; eauto.
+Qed.    
+
+Lemma wf_defs_intro : forall ids1 F lc,
+  (forall id1, In id1 ids1 ->
+   exists t1, exists gvs1,
+     lookupTypViaIDFromFdef F id1 = Some t1 /\
+     lookupAL _ lc id1 = Some gvs1 /\
+     wf_GVs gvs1 t1) ->
+  wf_defs F lc ids1.
+Proof.
+  induction ids1; intros.
+    apply wf_defs_nil.  
+
+    destruct (@H a) as [t1 [gvs1 [J1 [J2 J3]]]]; simpl; auto.
+    eapply wf_defs_cons; eauto.
+      apply IHids1.
+      intros id1 J.
+      apply H. simpl. auto.
+Qed.
+
+Lemma wf_defs_eq : forall ids2 ids1 F' lc',
+  set_eq _ ids1 ids2 ->
+  wf_defs F' lc' ids1 ->
+  wf_defs F' lc' ids2.
+Proof.
+  intros.
+  apply wf_defs_intro.
+  intros id1 Hin.
+  destruct H as [J1 J2].
+  eapply wf_defs_elim in H0; eauto.
+Qed.
+
+Lemma wf_defs_updateAddAL : forall g F' lc' ids1 ids2 i1 t1,
+  wf_defs F' lc' ids1 ->
+  set_eq _ (i1::ids1) ids2 ->
+  lookupTypViaIDFromFdef F' i1 = ret t1 ->
+  wf_GVs g t1 ->
+  wf_defs F' (updateAddAL _ lc' i1 g) ids2.
+Proof.
+  intros g F' lc' ids1 ids2 i1 t1 HwfDefs Heq Hlkup Hwfgvs.  
+  apply wf_defs_intro.  
+  intros id1 Hin.
+  destruct Heq as [Hinc1 Hinc2].
+  apply Hinc2 in Hin.
+  simpl in Hin.
+  destruct (eq_dec i1 id1); subst.
+    exists t1. exists g. 
+    split; auto.
+    split; auto. 
+      apply lookupAL_updateAddAL_eq; auto.      
+
+    destruct Hin as [Eq | Hin]; subst; try solve [contradict n; auto].
+    eapply wf_defs_elim in HwfDefs; eauto.
+    destruct HwfDefs as [t2 [gv2 [J1 [J2 J3]]]].
+    exists t2. exists gv2.
+    split; auto.
+    split; auto. 
+      rewrite <- lookupAL_updateAddAL_neq; auto.      
+Qed.
+
+Definition wf_lc (lc:GVsMap) : Prop :=
+forall i0 gvs0, lookupAL _ lc i0 = Some gvs0 -> Ensembles.Inhabited _ gvs0. 
+
+Lemma gv2gvs__inhabited : forall gv, 
+  Ensembles.Inhabited GenericValue ($ gv $).
+Proof.
+  intros gv.
+  apply Ensembles.Inhabited_intro with (x:=gv).
+  apply gv_in_gv2gvs.
+Qed.
+
+Lemma ogv2gvs__inhabited : forall ogv gvs,
+  %ogv% = ret gvs ->
+  Ensembles.Inhabited GenericValue gvs.
+Proof.
+  destruct ogv; intros; inv H.
+    apply gv2gvs__inhabited.
+Qed.
+
+Lemma getOperandValue__inhabited : forall TD v lc gl gvs,
+  wf_lc lc ->
+  NDopsem.getOperandValue TD v lc gl = Some gvs ->
+  Ensembles.Inhabited _ gvs.
+Proof.
+  intros TD v lc gl gvs Hwflc Hget.
+  destruct v; simpl in Hget; eauto using ogv2gvs__inhabited.
+Qed.
+    
+Lemma getIncomingValuesForBlockFromPHINodes_spec1 : forall ps TD b gl lc lc'
+    id1,
+  wf_lc lc ->
+  Some lc' = NDopsem.getIncomingValuesForBlockFromPHINodes TD ps b gl lc ->
+  In id1 (getPhiNodesIDs ps) ->
+  exists gvs, lookupAL _ lc' id1 = Some gvs /\ Ensembles.Inhabited _ gvs.  
+Proof.    
+  induction ps; intros TD b gl lc lc' id1 Hwflc H H0; simpl in *.
+    inversion H0.
+
+    destruct a.
+    simpl in H0.
+    destruct H0 as [H0 | H0]; subst.
+      destruct (getValueViaBlockFromValuels l0 b); try solve [inversion H].   
+        remember (NDopsem.getOperandValue TD v lc gl) as R.
+        destruct R; inversion H; subst. 
+        symmetry in HeqR. apply getOperandValue__inhabited in HeqR; auto.
+        destruct (NDopsem.getIncomingValuesForBlockFromPHINodes TD ps b gl 
+          lc); inversion H1; subst.         
+        exists g. simpl. 
+        destruct (id1==id1); auto.
+          contradict n; auto.
+
+      destruct (getValueViaBlockFromValuels l0 b); 
+        try solve [inversion H].   
+        remember (NDopsem.getOperandValue TD v lc gl) as R.
+        destruct R; inversion H; subst. 
+        symmetry in HeqR. apply getOperandValue__inhabited in HeqR; auto.
+        remember (NDopsem.getIncomingValuesForBlockFromPHINodes TD ps b gl 
+          lc) as R.
+        destruct R; inversion H2; subst.         
+        simpl.
+        destruct (id1==i0); subst; eauto.
+Qed.
+    
+Lemma updateValuesForNewBlock_spec1 : forall rs lc id1 gv,
+  lookupAL _ rs id1 = Some gv ->
+  lookupAL _ (NDopsem.updateValuesForNewBlock rs lc) id1 = Some gv.
+Proof.  
+  induction rs; intros; simpl in *.   
+    inversion H.
+
+    destruct a.
+    destruct (id1==a); subst.
+      inversion H; subst. apply lookupAL_updateAddAL_eq; auto.
+      rewrite <- lookupAL_updateAddAL_neq; auto.
+Qed.
+
+Ltac tinv H := try solve [inv H].
+
+Lemma getIncomingValuesForBlockFromPHINodes_spec2 : forall TD b gl lc 
+  (Hwflc: wf_lc lc) ps rs,
+  Some rs = NDopsem.getIncomingValuesForBlockFromPHINodes TD ps b gl lc ->
+  (forall id0 gvs, In (id0,gvs) rs -> Ensembles.Inhabited _ gvs).
+Proof.    
+  induction ps; intros rs H id0 gvs Hin; simpl in *.
+    inv H. inv Hin.
+
+    destruct a.
+    destruct (getValueViaBlockFromValuels l0 b); try solve [inversion H].   
+      remember (NDopsem.getOperandValue TD v lc gl) as R.
+      destruct R; tinv H.
+      symmetry in HeqR. apply getOperandValue__inhabited in HeqR; auto.
+      destruct (NDopsem.getIncomingValuesForBlockFromPHINodes TD ps b gl 
+        lc); inv H.
+      simpl in Hin. 
+      destruct Hin as [Hin | Hin]; eauto.
+        inv Hin; auto.
+Qed.
+
+Lemma updateValuesForNewBlock_spec2 : forall lc id1 gv,
+  lookupAL _ lc id1 = Some gv ->
+  wf_lc lc ->
+  forall rs, 
+  (forall id0 gvs, In (id0,gvs) rs -> Ensembles.Inhabited _ gvs) ->
+  exists gv', 
+    lookupAL _ (NDopsem.updateValuesForNewBlock rs lc) id1 = Some gv' /\
+    Ensembles.Inhabited _ gv'. 
+Proof.  
+  induction rs; intros; simpl in *.   
+    exists gv. eauto.
+
+    destruct a. 
+    destruct (id1==i0); subst.
+      exists e. rewrite lookupAL_updateAddAL_eq; eauto.
+      rewrite <- lookupAL_updateAddAL_neq; eauto.
+Qed.
+
+Lemma updateValuesForNewBlock_spec3 : forall lc,
+  wf_lc lc ->
+  forall rs, 
+  (forall id0 gvs, In (id0,gvs) rs -> Ensembles.Inhabited _ gvs) ->
+  wf_lc (NDopsem.updateValuesForNewBlock rs lc).
+Proof.  
+  induction rs; intros; simpl in *; auto.
+
+    destruct a.
+    intros x gvx Hlk.
+    destruct (i0==x); subst.
+      rewrite lookupAL_updateAddAL_eq in Hlk. inv Hlk. eauto.
+
+      rewrite <- lookupAL_updateAddAL_neq in Hlk; auto.
+      apply IHrs in Hlk; auto.
+        intros. eauto.
+Qed.
+
+Lemma wf_lc_br_aux : forall TD b1 b2 gl lc lc' 
+  (Hswitch : NDopsem.switchToNewBasicBlock TD b1 b2 gl lc = ret lc')
+  (Hwflc : wf_lc lc),
+  wf_lc lc'.
+Proof.
+  intros.
+  unfold NDopsem.switchToNewBasicBlock in Hswitch. simpl in Hswitch.
+  remember (NDopsem.getIncomingValuesForBlockFromPHINodes TD
+              (getPHINodesFromBlock b1) b2 gl lc) as R1.
+  destruct R1; inv Hswitch.
+  apply updateValuesForNewBlock_spec3; auto.
+    eapply getIncomingValuesForBlockFromPHINodes_spec2; eauto.
+Qed.
+
+Lemma wf_defs_br_aux : forall lc l' ps' cs' lc' F tmn' gl TD
+  (l3 : l)
+  (ps : phinodes)
+  (cs : list cmd) tmn
+  (Hlkup : Some (block_intro l' ps' cs' tmn') = lookupBlockViaLabelFromFdef F l')
+  (Hswitch : NDopsem.switchToNewBasicBlock TD (block_intro l' ps' cs' tmn')
+         (block_intro l3 ps cs tmn) gl lc = ret lc')
+  (t : list atom)
+  (Hwflc : wf_lc lc)
+  (Hwfdfs : wf_defs F lc t)
+  (ids0' : list atom)
+  (Hinc : incl (ListSet.set_diff eq_atom_dec ids0' (getPhiNodesIDs ps')) t),
+  wf_defs F lc' ids0'.
+Proof.
+  intros.
+  unfold NDopsem.switchToNewBasicBlock in Hswitch. simpl in Hswitch.
+  remember (NDopsem.getIncomingValuesForBlockFromPHINodes TD ps'
+                (block_intro l3 ps cs tmn) gl lc) as R1.
+  destruct R1; inv Hswitch.
+  apply wf_defs_intro.
+  intros id1 Hid1.
+  destruct (In_dec eq_atom_dec id1 (getPhiNodesIDs ps')) as [Hin | Hnotin].
+    eapply getIncomingValuesForBlockFromPHINodes_spec1 in HeqR1; eauto.
+    destruct HeqR1 as [gv [HeqR1 Hinh]].
+    apply updateValuesForNewBlock_spec1 with (lc:=lc) in HeqR1.
+    eapply InPhiNodes_lookupTypViaIDFromFdef in Hlkup; eauto.
+    destruct Hlkup as [t1 Hlkup].
+    exists t1. exists gv.
+    split; auto.
+
+    apply ListSet.set_diff_intro with (x:=ids0')(Aeq_dec:=eq_atom_dec) in Hnotin;
+      auto.
+    apply Hinc in Hnotin.
+    apply wf_defs_elim with (id1:=id1) in Hwfdfs; auto.
+    destruct Hwfdfs as [t1 [gv1 [J1 [J2 J3]]]].
+    apply updateValuesForNewBlock_spec2 with (rs:=l0) in J2; auto.
+      destruct J2 as [gv' [J2 J2']].
+      exists t1. exists gv'. 
+      split; auto.
+
+      eapply getIncomingValuesForBlockFromPHINodes_spec2; eauto.
+Qed.
+
+Lemma inscope_of_tmn_br_aux : forall F l3 ps cs tmn ids0 l' ps' cs' tmn' l0 ifs
+  s m lc lc' TD gl,
+wf_lc lc ->
+wf_fdef ifs s m F ->
+uniqFdef F ->
+blockInFdefB (block_intro l3 ps cs tmn) F = true ->
+In l0 (successors_terminator tmn) ->
+Some ids0 = inscope_of_tmn F (block_intro l3 ps cs tmn) tmn ->
+Some (block_intro l' ps' cs' tmn') = lookupBlockViaLabelFromFdef F l0 ->
+NDopsem.switchToNewBasicBlock TD (block_intro l' ps' cs' tmn')
+  (block_intro l3 ps cs tmn) gl lc = Some lc' ->
+wf_defs F lc ids0 ->
+exists ids0',
+  match cs' with
+  | nil => Some ids0' = inscope_of_tmn F (block_intro l' ps' cs' tmn') tmn'
+  | c'::_ => Some ids0' = inscope_of_cmd F (block_intro l' ps' cs' tmn') c'
+  end /\
+  incl (ListSet.set_diff eq_atom_dec ids0' (getPhiNodesIDs ps')) ids0 /\
+  wf_defs F lc' ids0'.
+Proof.
+  intros F l3 ps cs tmn ids0 l' ps' cs' tmn' l0 ifs s m lc lc' TD gl Hwflc HwfF 
+    Huniq HBinF Hsucc Hinscope Hlkup Hswitch Hwfdfs.
+  symmetry in Hlkup.
+  assert (J:=Hlkup).
+  apply lookupBlockViaLabelFromFdef_inv in J; auto.
+  destruct J as [Heq J]; subst.
+  unfold inscope_of_tmn in Hinscope.
+  unfold inscope_of_tmn. unfold inscope_of_cmd.
+  destruct F as [[? ? ? la va] bs].
+  remember (dom_analyze (fdef_intro (fheader_intro f t i0 la va) bs)) as Doms.
+  remember (Doms !! l3)as defs3.
+  remember (Doms !! l')as defs'.
+  destruct defs3 as [contents3 inbound3]. 
+  destruct defs' as [contents' inbound']. 
+
+  assert (incl contents' (l3::contents3)) as Hsub.
+    clear - HBinF Hsucc Heqdefs3 Heqdefs' HeqDoms Huniq HwfF.
+    simpl in Huniq. destruct Huniq.
+    eapply dom_successors; eauto.
+
+  destruct cs'.
+  Case "cs'=nil".
+    assert (J1:=inbound').
+    apply fold_left__bound_blocks with (init:=getPhiNodesIDs ps' ++ 
+      getCmdsIDs nil ++ getArgsIDs la)(t:=t)(i0:=i0)(la:=la)(va:=va)(bs:=bs)
+      (fa:=f)(l0:=l') in J1.
+    destruct J1 as [r J1].
+    exists r. split; auto.
+
+    assert (incl (ListSet.set_diff eq_atom_dec r (getPhiNodesIDs ps')) ids0)
+      as Jinc.
+      clear - Hinscope J1 Hsub HBinF Huniq.
+      apply fold_left__spec in J1.
+      symmetry in Hinscope.
+      apply fold_left__spec in Hinscope.
+      destruct J1 as [J1 [J2 J3]].
+      destruct Hinscope as [J4 [J5 J6]].
+      intros id1 J.
+      assert (J':=J).
+      apply ListSet.set_diff_elim1 in J.
+      apply ListSet.set_diff_elim2 in J'.
+      apply J3 in J.
+      destruct J as [J | J].
+      SCase "id1 in init and the current block".
+        simpl in J.
+        apply in_app_or in J.
+        destruct J as [J | J]; try solve [contradict J; auto].
+        apply J4.
+        apply in_or_app. right.
+        apply in_or_app; auto.
+      SCase "id1 in strict dominating blocks".
+        destruct J as [b1 [l1 [J8 [J9 J10]]]].
+        assert (In l1 contents') as J8'.
+          clear - J8.
+          apply ListSet.set_diff_elim1 in J8. auto.
+        apply Hsub in J8'.
+          destruct (eq_atom_dec l1 l3); subst.
+            simpl in J9. 
+            assert (b1=block_intro l3 ps cs tmn) as EQ.
+              clear - J9 HBinF Huniq. destruct Huniq.
+              eapply InBlocksB__lookupAL; eauto.
+            subst.
+            simpl in J10.
+            apply J4.
+            rewrite_env 
+              ((getPhiNodesIDs ps ++ getCmdsIDs cs) ++ getArgsIDs la).
+            apply in_or_app; auto.
+      
+            apply J5 in J9; auto.
+              simpl in J8'.
+              destruct J8' as [J8' | J8']; try solve [contradict n; auto].
+              apply ListSet.set_diff_intro; auto.
+                intro J. simpl in J. 
+                destruct J as [J | J]; auto.
+
+    split; auto.
+      eauto using wf_defs_br_aux.
+        
+  Case "cs'<>nil".
+    assert (J1:=inbound').
+    unfold cmds_dominates_cmd. simpl.
+    destruct (eq_atom_dec (getCmdLoc c) (getCmdLoc c)) as [_ | n]; 
+      try solve [contradict n; auto].
+    simpl_env.
+    apply fold_left__bound_blocks with (init:=getPhiNodesIDs ps' ++ 
+      getArgsIDs la)(t:=t)(i0:=i0)(la:=la)(va:=va)(bs:=bs)(l0:=l')(fa:=f) in J1.
+    destruct J1 as [r J1].
+    exists r.  split; auto.
+
+    assert (incl (ListSet.set_diff eq_atom_dec r (getPhiNodesIDs ps')) ids0)
+      as Jinc.
+      clear - Hinscope J1 Hsub HBinF Huniq.
+      apply fold_left__spec in J1.
+      symmetry in Hinscope.
+      apply fold_left__spec in Hinscope.
+      destruct J1 as [J1 [J2 J3]].
+      destruct Hinscope as [J4 [J5 J6]].
+      intros id1 J.
+      assert (J':=J).
+      apply ListSet.set_diff_elim1 in J.
+      apply ListSet.set_diff_elim2 in J'.
+      apply J3 in J.
+      destruct J as [J | J].
+      SCase "id1 in init and the current block".
+        simpl in J.
+        apply in_app_or in J.
+        destruct J as [J | J]; try solve [contradict J; auto].
+        apply J4.
+        apply in_or_app. right.
+        apply in_or_app; auto.
+      SCase "id1 in strict dominating blocks".
+        destruct J as [b1 [l1 [J8 [J9 J10]]]].
+        assert (In l1 contents') as J8'.
+          clear - J8.
+          apply ListSet.set_diff_elim1 in J8. auto.
+        apply Hsub in J8'.
+          destruct (eq_atom_dec l1 l3); subst.
+            simpl in J9. 
+            assert (b1=block_intro l3 ps cs tmn) as EQ.
+              clear - J9 HBinF Huniq. destruct Huniq.
+              eapply InBlocksB__lookupAL; eauto.
+            subst.
+            simpl in J10.
+            apply J4.
+            rewrite_env 
+              ((getPhiNodesIDs ps ++ getCmdsIDs cs) ++ getArgsIDs la).
+            apply in_or_app; auto.
+      
+            apply J5 in J9; auto. 
+              simpl in J8'.
+              destruct J8' as [J8' | J8']; try solve [contradict n; auto].
+              apply ListSet.set_diff_intro; auto.
+                intro J. simpl in J. 
+                destruct J as [J | J]; auto.
+
+    split; auto.
+      eauto using wf_defs_br_aux.
+Qed.
+
+Lemma inscope_of_tmn_br_uncond : forall F l3 ps cs bid ids0 l' ps' cs' tmn' l0 
+ ifs s m gl lc lc' TD,
+wf_lc lc ->
+wf_fdef ifs s m F ->
+uniqFdef F ->
+blockInFdefB (block_intro l3 ps cs (insn_br_uncond bid l0)) F = true ->
+Some ids0 = inscope_of_tmn F (block_intro l3 ps cs (insn_br_uncond bid l0)) 
+  (insn_br_uncond bid l0) ->
+Some (block_intro l' ps' cs' tmn') = lookupBlockViaLabelFromFdef F l0 ->
+NDopsem.switchToNewBasicBlock TD (block_intro l' ps' cs' tmn')
+  (block_intro l3 ps cs (insn_br_uncond bid l0)) gl lc = Some lc' ->
+wf_defs F lc ids0 ->
+exists ids0',
+  match cs' with
+  | nil => Some ids0' = inscope_of_tmn F (block_intro l' ps' cs' tmn') tmn'
+  | c'::_ => Some ids0' = inscope_of_cmd F (block_intro l' ps' cs' tmn') c'
+  end /\
+  incl (ListSet.set_diff eq_atom_dec ids0' (getPhiNodesIDs ps')) ids0 /\
+  wf_defs F lc' ids0'.
+Proof.
+  intros.
+  eapply inscope_of_tmn_br_aux; eauto.
+  simpl. auto.
+Qed.
+
+Lemma inscope_of_tmn_br : forall F l0 ps cs bid l1 l2 ids0 l' ps' cs' tmn' Cond 
+  c TD gl lc ifs s m lc',
+wf_lc lc ->
+wf_fdef ifs s m F ->
+uniqFdef F ->
+blockInFdefB (block_intro l0 ps cs (insn_br bid Cond l1 l2)) F = true ->
+Some ids0 = inscope_of_tmn F (block_intro l0 ps cs (insn_br bid Cond l1 l2)) 
+  (insn_br bid Cond l1 l2) ->
+Some (block_intro l' ps' cs' tmn') =
+       (if isGVZero TD c
+        then lookupBlockViaLabelFromFdef F l2
+        else lookupBlockViaLabelFromFdef F l1) ->
+NDopsem.switchToNewBasicBlock TD (block_intro l' ps' cs' tmn')
+  (block_intro l0 ps cs (insn_br bid Cond l1 l2)) gl lc = Some lc' ->
+wf_defs F lc ids0 ->
+exists ids0',
+  match cs' with
+  | nil => Some ids0' = inscope_of_tmn F (block_intro l' ps' cs' tmn') tmn'
+  | c'::_ => Some ids0' = inscope_of_cmd F (block_intro l' ps' cs' tmn') c'
+  end /\
+  incl (ListSet.set_diff eq_atom_dec ids0' (getPhiNodesIDs ps')) ids0 /\
+  wf_defs F lc' ids0'.
+Proof.
+  intros.
+  remember (isGVZero TD c) as R.
+  destruct R; eapply inscope_of_tmn_br_aux; eauto; simpl; auto.
+Qed.
+
+Lemma params2GVs_inhabited : forall TD gl lc (Hwfc : wf_lc lc) lp gvs,
+  NDopsem.params2GVs TD lp lc gl = Some gvs ->
+  (forall gv, In gv gvs -> Ensembles.Inhabited _ gv).
+Proof.
+  induction lp; simpl; intros gvs Hp2gv gv Hin.
+    inv Hp2gv. inv Hin.
+
+    destruct a. 
+    remember (NDopsem.getOperandValue TD v lc gl) as R0.
+    destruct R0; try solve [inv Hp2gv].
+    remember (NDopsem.params2GVs TD lp lc gl) as R.
+    destruct R; inv Hp2gv.
+    simpl in Hin.
+    destruct Hin as [Hin | Hin]; subst; eauto.
+      eapply getOperandValue__inhabited; eauto.
+Qed.
+
+Lemma initLocals_spec' : forall la gvs id1,
+  In id1 (getArgsIDs la) ->
+  exists gv, lookupAL _ (NDopsem.initLocals la gvs) id1 = Some gv.
+Proof.
+  unfold NDopsem.initLocals.
+  induction la; intros; simpl in *.
+    inversion H.
+
+    destruct a.  
+    simpl in H.
+    destruct H as [H | H]; subst; simpl.
+      destruct gvs. 
+        exists (Ensembles.Full_set _). apply lookupAL_updateAddAL_eq; auto.      
+        exists g. apply lookupAL_updateAddAL_eq; auto.      
+
+      destruct (eq_atom_dec i0 id1); subst.
+        destruct gvs.
+          exists (Ensembles.Full_set _). apply lookupAL_updateAddAL_eq; auto.
+          exists g. apply lookupAL_updateAddAL_eq; auto.
+        destruct gvs; rewrite <- lookupAL_updateAddAL_neq; auto.
+Qed.
+
+Lemma wf_lc_updateAddAL : forall lc gv i0,
+  wf_lc lc -> Ensembles.Inhabited _ gv -> wf_lc (updateAddAL _ lc i0 gv).
+Proof.
+  intros.
+  intros x gvx Hlk.
+  destruct (eq_atom_dec i0 x); subst.
+    rewrite lookupAL_updateAddAL_eq in Hlk.
+    inv Hlk. auto.
+
+    rewrite <- lookupAL_updateAddAL_neq in Hlk; eauto.
+Qed.
+
+Lemma initializeFrameValues__wf_lc : forall lc1 (Hwflc:wf_lc lc1) la2 gvs2,
+  (forall gv, In gv gvs2 -> Ensembles.Inhabited _ gv) ->
+  wf_lc (NDopsem._initializeFrameValues la2 gvs2 lc1).
+Proof.
+  induction la2; simpl; intros gvs2 Hin; auto.
+    destruct a.
+    destruct gvs2; simpl in *; subst.
+      apply wf_lc_updateAddAL; eauto.
+        apply full_set_inhabited.
+      apply wf_lc_updateAddAL; eauto.
+Qed.
+
+Lemma initLocals__wf_lc : forall la gvs,
+  (forall gv, In gv gvs -> Ensembles.Inhabited _ gv) ->  
+  wf_lc (NDopsem.initLocals la gvs).
+Proof.
+  intros. unfold NDopsem.initLocals. 
+  apply initializeFrameValues__wf_lc; auto.
+    intros x gvx J. inv J.
+Qed.
+
+Lemma initLocals_spec : forall la gvs id1,
+  (forall gv, In gv gvs -> Ensembles.Inhabited _ gv) ->  
+  In id1 (getArgsIDs la) ->
+  exists gv, lookupAL _ (NDopsem.initLocals la gvs) id1 = Some gv /\
+    Ensembles.Inhabited _ gv.
+Proof.
+  intros.
+  apply initLocals_spec' with (gvs:=gvs) in H0; auto.
+  destruct H0 as [gv H0].
+  exists gv. split; auto.
+  apply initLocals__wf_lc with (la:=la) in H; eauto.
+Qed.
+
+Lemma returnUpdateLocals__wf_lc : forall TD c Result lc lc' gl lc'',
+  wf_lc lc -> wf_lc lc' ->
+  NDopsem.returnUpdateLocals TD c Result lc lc' gl = ret lc'' ->
+  wf_lc lc''.
+Proof.
+  intros.
+  unfold NDopsem.returnUpdateLocals in H1.
+  remember (NDopsem.getOperandValue TD Result lc gl) as R.
+  destruct R; tinv H1.
+  destruct (getCallerReturnID c); inv H1; auto.
+    apply wf_lc_updateAddAL; eauto using getOperandValue__inhabited.
+Qed.
+
+Lemma lift_op2__inhabited : forall f gvs1 gvs2 
+  (H:forall x y, exists z, f x y = Some z),
+  Ensembles.Inhabited _ gvs1 -> Ensembles.Inhabited _ gvs2 ->
+  Ensembles.Inhabited _ (lift_op2 f gvs1 gvs2).
+Proof.
+  intros.
+  unfold lift_op2. 
+  inv H0. inv H1.
+  destruct (@H x x0) as [z J].
+  exists z. unfold Ensembles.In. exists x. exists x0. exists z.
+  rewrite J.
+  repeat (split; auto).
+    apply gv_in_gv2gvs.
+Qed.
+
+Lemma mbop_is_total : forall TD bop0 sz0 x y, 
+  exists z, mbop TD bop0 sz0 x y = Some z.
+Proof.
+  intros.
+  unfold mbop.
+  destruct (GV2val TD x); eauto.
+  destruct v; eauto.
+  destruct (GV2val TD y); eauto.
+  destruct v; eauto.
+  destruct (eq_nat_dec (wz + 1) (Size.to_nat sz0)); eauto.
+  destruct bop0; eauto.
+Qed.
+
+Lemma BOP__inhabited : forall TD lc gl bop0 sz0 v1 v2 gvs3,
+  wf_lc lc ->
+  NDopsem.BOP TD lc gl bop0 sz0 v1 v2 = ret gvs3 ->
+  Ensembles.Inhabited GenericValue gvs3.
+Proof.
+  intros TD lc gl bop0 sz0 v1 v2 gvs3 Hwflc Hbop.
+  unfold NDopsem.BOP in Hbop.
+  remember(NDopsem.getOperandValue TD v1 lc gl) as R1.
+  destruct R1; tinv Hbop.
+  remember(NDopsem.getOperandValue TD v2 lc gl) as R2.
+  destruct R2; inv Hbop.
+  apply lift_op2__inhabited; eauto using getOperandValue__inhabited.
+  apply mbop_is_total; auto.
+Qed.
+
+Lemma values2GVs__inhabited' : forall TD lc (Hwflc: wf_lc lc) gl idxs vidxs,
+  NDopsem.values2GVs TD idxs lc gl = Some vidxs ->
+  (forall gvs, In gvs vidxs -> Ensembles.Inhabited GenericValue gvs).
+Proof.
+  induction idxs; simpl; intros vidxs Hv2gvs gvs Hin.
+    inv Hv2gvs. inv Hin.
+
+    remember (NDopsem.getOperandValue TD v lc gl) as R.
+    destruct R; tinv Hv2gvs.
+    remember (NDopsem.values2GVs TD idxs lc gl) as R1.
+    destruct R1; inv Hv2gvs.
+    simpl in Hin.
+    destruct Hin as [Hin | Hin]; subst; eauto.
+      eauto using getOperandValue__inhabited.
+Qed.
+
+Lemma values2GVs__inhabited : forall TD lc (Hwflc: wf_lc lc) gl idxs vidxs,
+  NDopsem.values2GVs TD idxs lc gl = Some vidxs ->
+  exists vidxs0, vidxs0 @@ vidxs.
+Proof.
+  induction idxs; simpl; intros vidxs Hv2gvs.
+    inv Hv2gvs. exists nil. simpl. auto.
+
+    remember (NDopsem.getOperandValue TD v lc gl) as R.
+    destruct R; tinv Hv2gvs.
+    remember (NDopsem.values2GVs TD idxs lc gl) as R1.
+    destruct R1; inv Hv2gvs.
+    symmetry in HeqR1. symmetry in HeqR.
+    destruct (@IHidxs l0) as [vidxs0 J]; auto.
+    apply getOperandValue__inhabited in HeqR; auto.
+    inv HeqR.
+    exists (x::vidxs0). simpl. simpl; auto.
+Qed.
+
+Lemma GEP_is_total : forall TD t mp vidxs inbounds0,
+  exists mp', GEP TD t mp vidxs inbounds0 = ret mp'.
+Proof.
+  intros. unfold GEP.
+  destruct (GV2ptr TD (getPointerSize TD) mp); eauto.
+  destruct (GVs2Nats TD vidxs); eauto.
+  destruct (mgep TD t v l0); eauto.
+Qed.
+
+Lemma GEP__inhabited : forall TD t mp vidxs inbounds0 mp' vidxs0,
+  Ensembles.Inhabited GenericValue mp ->
+  vidxs0 @@ vidxs ->
+  NDopsem.GEP TD t mp vidxs inbounds0 = ret mp' ->
+  Ensembles.Inhabited GenericValue mp'.
+Proof.
+  intros.
+  unfold NDopsem.GEP in H1. inv H1.
+  inv H.
+  destruct (@GEP_is_total TD t x vidxs0 inbounds0) as [mp' J].
+  apply Ensembles.Inhabited_intro with (x:=mp').
+  unfold Ensembles.In.
+  exists x. exists vidxs0. rewrite J. split; auto.
+Qed.
+
+
+Lemma lift_op1__inhabited : forall f gvs1
+  (H:forall x, exists z, f x = Some z),
+  Ensembles.Inhabited _ gvs1 ->
+  Ensembles.Inhabited _ (lift_op1 f gvs1).
+Proof.
+  intros.
+  unfold lift_op1. 
+  inv H0.
+  destruct (@H x) as [z J].
+  exists z. unfold Ensembles.In. exists x. exists z.
+  rewrite J.
+  repeat (split; auto).
+    apply gv_in_gv2gvs.
+Qed.
+
+Lemma mcast_is_total : forall TD cop0 t1 t2 x, 
+  exists z, mcast TD cop0 t1 t2 x = Some z.
+Proof.
+  intros.
+  unfold mcast, mbitcast.
+  destruct cop0; destruct t1; destruct t2; eauto.
+Qed.
+
+Lemma CAST__inhabited : forall TD lc gl cop0 t1 v1 t2 gvs2,
+  wf_lc lc ->
+  NDopsem.CAST TD lc gl cop0 t1 v1 t2 = ret gvs2 ->
+  Ensembles.Inhabited GenericValue gvs2.
+Proof.
+  intros TD lc gl cop0 t1 v1 t2 gvs2 Hwflc Hcast.
+  unfold NDopsem.CAST in Hcast.
+  remember(NDopsem.getOperandValue TD v1 lc gl) as R1.
+  destruct R1; inv Hcast.
+  apply lift_op1__inhabited; eauto using getOperandValue__inhabited.
+  apply mcast_is_total; auto.
+Qed.
+
+(*********************************************)
+(** * Preservation *)
+
+Lemma preservation_dbCall_case : forall fid l' fa rt la va lb bs_contents gvs
+  (Hinhs : forall gv, In gv gvs -> Ensembles.Inhabited _ gv)
+  (bs_bound : incl bs_contents (bound_blocks lb))
+  (H0 : incl bs_contents [l']),
+   match
+     fold_left
+       (inscope_of_block (fdef_intro (fheader_intro fa rt fid la va) lb) l')
+       bs_contents (ret getArgsIDs la)
+   with
+   | ret ids0 =>
+       wf_defs (fdef_intro (fheader_intro fa rt fid la va) lb)
+         (NDopsem.initLocals la gvs) ids0
+   | merror => False
+   end.
+Proof.
+  intros.
+  assert (J:=bs_bound).
+  apply fold_left__bound_blocks with (t:=rt)(i0:=fid)(la:=la)(va:=va)(fa:=fa)
+    (l0:=l')(init:=getArgsIDs la) in J.
+  destruct J as [r J].
+  rewrite J.       
+  apply fold_left__spec in J.
+  destruct J as [_ [_ J]].
+  apply wf_defs_intro.
+  intros id1 Hin.
+  apply J in Hin.
+  destruct Hin as [Hin | Hin].    
+    assert (J1:=Hin).
+    apply InArgsIDs_lookupTypViaIDFromFdef with (t0:=rt)(id0:=fid)(la0:=la)
+      (va0:=va)(bs:=lb)(fa:=fa) in J1.
+    destruct J1 as [t J1].
+    exists t. rewrite J1.
+    apply initLocals_spec with (gvs:=gvs) in Hin; auto.
+    destruct Hin as [gv [Hin Hinh]].
+    exists gv. split; auto.
+  
+    destruct Hin as [b1 [l1 [Hin _]]].
+    simpl in H0. clear - H0 Hin.
+    assert (J:=Hin).
+    apply ListSet.set_diff_elim1 in Hin.
+    apply ListSet.set_diff_elim2 in J.
+    apply H0 in Hin.
+    simpl in Hin. 
+    destruct Hin as [Hin | Hin]; subst; try inversion Hin.
+    simpl in J. contradict J; auto.
+Qed.
+
+Definition wf_ExecutionContext (ps:list product) 
+  (ec:NDopsem.ExecutionContext) : Prop :=
+let '(NDopsem.mkEC f b cs tmn lc als) := ec in
+isReachableFromEntry f b /\
+blockInFdefB b f = true /\
+InProductsB (product_fdef f) ps = true /\
+wf_lc lc /\
+match cs with
+| nil => 
+    match inscope_of_tmn f b tmn with
+    | Some ids => wf_defs f lc ids
+    | None => False
+    end
+| c::_ =>
+    match inscope_of_cmd f b c with
+    | Some ids => wf_defs f lc ids
+    | None => False
+    end
+end /\
+exists l1, exists ps, exists cs',
+b = block_intro l1 ps (cs'++cs) tmn.
+
+Definition wf_call (ec:NDopsem.ExecutionContext) (ecs:NDopsem.ECStack) 
+  : Prop :=
+let '(NDopsem.mkEC f _ _ _ _ _) := ec in
+forall b, blockInFdefB b f ->
+let '(block_intro _ _ _ tmn) := b in
+match tmn with
+| insn_return _ _ _ | insn_return_void _ =>
+    match ecs with
+    | nil => True
+    | NDopsem.mkEC f' b' (insn_call _ _ _ _ _ _ ::_) tmn' lc' als'::ecs' 
+        => True
+    | _ => False
+    end
+| _ => True
+end.
+
+Fixpoint wf_ECStack (ps:list product) (ecs:NDopsem.ECStack) : Prop :=
+match ecs with
+| nil => False
+| ec::ecs' => wf_ExecutionContext ps ec /\ wf_ECStack ps ecs' /\ wf_call ec ecs'
+end.
+
+Definition wf_global system5 gl := forall id5 typ5, 
+  lookupTypViaGIDFromSystem system5 id5 = ret typ5 ->
+  exists gv : GenericValue, lookupAL GenericValue gl id5 = Some gv.
+
+Definition wf_State (S:NDopsem.State) : Prop :=
+let '(NDopsem.mkState s (los, nts) ps ecs gl _ _) := S in
+wf_global s gl /\
+wf_system nil s /\
+moduleInSystemB (module_intro los nts ps) s = true /\
+wf_ECStack ps ecs.
+
+Lemma preservation_cmd_updated_case : forall
+  (S : system)
+  (los : layouts)
+  (nts : namedts)
+  (Ps : list product)
+  (F : fdef)
+  (B : block)
+  (lc : GVsMap)
+  (gl : GVMap)
+  (fs : GVMap)
+  (gv3 : GVs)
+  (Hinhabited : Ensembles.Inhabited GenericValue gv3)
+  (EC : list NDopsem.ExecutionContext)
+  (cs : list cmd)
+  (tmn : terminator)
+  (Mem0 : mem)
+  (als : list mblock)
+  id0 c0
+  (Hid : Some id0 = getCmdID c0)
+  t0
+  (Htyp : Some t0 = getCmdTyp c0)
+  (HwfS1 : wf_State
+            {|
+            NDopsem.CurSystem := S;
+            NDopsem.CurTargetData := (los, nts);
+            NDopsem.CurProducts := Ps;
+            NDopsem.ECS := {|
+                   NDopsem.CurFunction := F;
+                   NDopsem.CurBB := B;
+                   NDopsem.CurCmds := c0 :: cs;
+                   NDopsem.Terminator := tmn;
+                   NDopsem.Locals := lc;
+                   NDopsem.Allocas := als |} :: EC;
+            NDopsem.Globals := gl;
+            NDopsem.FunTable := fs;
+            NDopsem.Mem := Mem0 |}),
+   wf_State
+     {|
+     NDopsem.CurSystem := S;
+     NDopsem.CurTargetData := (los, nts);
+     NDopsem.CurProducts := Ps;
+     NDopsem.ECS := {|
+            NDopsem.CurFunction := F;
+            NDopsem.CurBB := B;
+            NDopsem.CurCmds := cs;
+            NDopsem.Terminator := tmn;
+            NDopsem.Locals := updateAddAL GVs lc id0 gv3;
+            NDopsem.Allocas := als |} :: EC;
+     NDopsem.Globals := gl;
+     NDopsem.FunTable := fs;
+     NDopsem.Mem := Mem0 |}.
+Proof.
+  intros.
+  destruct HwfS1 as 
+    [Hwfg [HwfSystem [HmInS [
+     [Hreach1 [HBinF1 [HFinPs1 [Hwflc1 [Hinscope1 [l3 [ps3 [cs3' Heq1]]]]]]]]
+     [HwfEC HwfCall]]]]
+    ]; subst.
+  remember (inscope_of_cmd F (block_intro l3 ps3 (cs3' ++ c0 :: cs) tmn) c0) 
+    as R1. 
+  destruct R1; try solve [inversion Hinscope1].
+  repeat (split; try solve [auto]).
+      apply wf_lc_updateAddAL; auto.
+      assert (Hid':=Hid).
+      symmetry in Hid.
+      apply getCmdLoc_getCmdID in Hid.
+       subst.
+      destruct cs; simpl_env in *.
+      Case "1.1.1".
+        assert (~ In (getCmdLoc c0) (getCmdsLocs cs3')) as Hnotin.
+          eapply wf_system__uniq_block with (f:=F) in HwfSystem; eauto.        
+          simpl in HwfSystem.
+          apply NoDup_inv in HwfSystem.
+          destruct HwfSystem as [_ J].
+          apply NoDup_inv in J.
+          destruct J as [J _].
+          rewrite getCmdsLocs_app in J.
+          simpl in J.
+          apply NoDup_last_inv in J. auto.
+
+        apply inscope_of_cmd_tmn in HeqR1; auto.
+        destruct HeqR1 as [ids2 [J1 J2]].        
+        rewrite <- J1.
+        assert (In c0 (cs3' ++ [c0])) as HinCs.
+          apply in_or_app. right. simpl. auto.
+        assert (Hwfc := HBinF1).
+        eapply wf_system__wf_cmd with (c:=c0) in Hwfc; 
+          eauto.
+        rewrite <- Hid' in J2.
+        eapply wf_defs_updateAddAL with (t1:=t0) ; eauto.
+          eapply uniqF__lookupTypViaIDFromFdef; eauto.
+            eapply wf_system__uniqFdef; eauto.
+        
+      Case "1.1.2".
+        assert (NoDup (getCmdsLocs (cs3' ++ [c0] ++ [c] ++ cs))) as Hnodup.
+          eapply wf_system__uniq_block with (f:=F) in HwfSystem; eauto.        
+          simpl in HwfSystem.
+          apply NoDup_inv in HwfSystem.
+          destruct HwfSystem as [_ J].
+          apply NoDup_inv in J.
+          destruct J as [J _]. auto.
+        apply inscope_of_cmd_cmd in HeqR1; auto.
+        destruct HeqR1 as [ids2 [J1 J2]].        
+        rewrite <- J1.
+        assert (In c0 (cs3' ++ [c0] ++ [c] ++ cs)) as HinCs.
+          apply in_or_app. right. simpl. auto.
+        assert (Hwfc := HBinF1).
+        eapply wf_system__wf_cmd with (c:=c0) in Hwfc; 
+          eauto.
+        rewrite <- Hid' in J2.
+        eapply wf_defs_updateAddAL with (t1:=t0) ; eauto.
+          eapply uniqF__lookupTypViaIDFromFdef; eauto.
+            eapply wf_system__uniqFdef; eauto.
+
+  exists l3. exists ps3. exists (cs3'++[c0]). simpl_env. auto.
+Qed.
+
+Lemma preservation_cmd_non_updated_case : forall
+  (S : system)
+  (los : layouts)
+  (nts : namedts)
+  (Ps : list product)
+  (F : fdef)
+  (B : block)
+  (lc : GVsMap)
+  (gl : GVMap)
+  (fs : GVMap)
+  (EC : list NDopsem.ExecutionContext)
+  (cs : list cmd)
+  (tmn : terminator)
+  (Mem0 : mem)
+  (als : list mblock)
+  c0
+  (Hid : getCmdID c0 = None)
+  (HwfS1 : wf_State
+            {|
+            NDopsem.CurSystem := S;
+            NDopsem.CurTargetData := (los, nts);
+            NDopsem.CurProducts := Ps;
+            NDopsem.ECS := {|
+                   NDopsem.CurFunction := F;
+                   NDopsem.CurBB := B;
+                   NDopsem.CurCmds := c0 :: cs;
+                   NDopsem.Terminator := tmn;
+                   NDopsem.Locals := lc;
+                   NDopsem.Allocas := als |} :: EC;
+            NDopsem.Globals := gl;
+            NDopsem.FunTable := fs;
+            NDopsem.Mem := Mem0 |}),
+   wf_State
+     {|
+     NDopsem.CurSystem := S;
+     NDopsem.CurTargetData := (los, nts);
+     NDopsem.CurProducts := Ps;
+     NDopsem.ECS := {|
+            NDopsem.CurFunction := F;
+            NDopsem.CurBB := B;
+            NDopsem.CurCmds := cs;
+            NDopsem.Terminator := tmn;
+            NDopsem.Locals := lc;
+            NDopsem.Allocas := als |} :: EC;
+     NDopsem.Globals := gl;
+     NDopsem.FunTable := fs;
+     NDopsem.Mem := Mem0 |}.
+Proof.
+  intros.
+  destruct HwfS1 as 
+    [Hwfg [HwfSystem [HmInS [
+     [Hreach1 [HBinF1 [HFinPs1 [Hwflc1 [Hinscope1 [l3 [ps3 [cs3' Heq1]]]]]]]]
+     [HwfEC HwfCall]]]]
+    ]; subst.
+  remember (inscope_of_cmd F (block_intro l3 ps3 (cs3' ++ c0 :: cs) tmn) c0) 
+    as R1. 
+  destruct R1; try solve [inversion Hinscope1].
+  repeat (split; try solve [auto]).
+      destruct cs; simpl_env in *.
+      Case "1.1.1".
+        assert (~ In (getCmdLoc c0) (getCmdsLocs cs3')) as Hnotin.
+          eapply wf_system__uniq_block with (f:=F) in HwfSystem; eauto.        
+          simpl in HwfSystem.
+          apply NoDup_inv in HwfSystem.
+          destruct HwfSystem as [_ J].
+          apply NoDup_inv in J.
+          destruct J as [J _].
+          rewrite getCmdsLocs_app in J.
+          simpl in J.
+          apply NoDup_last_inv in J. auto.
+
+        apply inscope_of_cmd_tmn in HeqR1; auto.
+        destruct HeqR1 as [ids2 [J1 J2]].        
+        rewrite <- J1.
+        assert (In c0 (cs3' ++ [c0])) as HinCs.
+          apply in_or_app. right. simpl. auto.
+        assert (Hwfc := HBinF1).
+        eapply wf_system__wf_cmd with (c:=c0) in Hwfc; 
+          eauto.
+        rewrite Hid in J2.
+        eapply wf_defs_eq; eauto.
+        
+      Case "1.1.2".
+        assert (NoDup (getCmdsLocs (cs3' ++ [c0] ++ [c] ++ cs))) as Hnodup.
+          eapply wf_system__uniq_block with (f:=F) in HwfSystem; eauto.        
+          simpl in HwfSystem.
+          apply NoDup_inv in HwfSystem.
+          destruct HwfSystem as [_ J].
+          apply NoDup_inv in J.
+          destruct J as [J _]. auto.
+        apply inscope_of_cmd_cmd in HeqR1; auto.
+        destruct HeqR1 as [ids2 [J1 J2]].        
+        rewrite <- J1.
+        assert (In c0 (cs3' ++ [c0] ++ [c] ++ cs)) as HinCs.
+          apply in_or_app. right. simpl. auto.
+        assert (Hwfc := HBinF1).
+        eapply wf_system__wf_cmd with (c:=c0) in Hwfc; 
+          eauto.
+        rewrite Hid in J2.
+        eapply wf_defs_eq ; eauto.
+
+  exists l3. exists ps3. exists (cs3'++[c0]). simpl_env. auto.
+Qed.
+
+Lemma wf_State__wf_lc : forall S TD Ps F B c cs tmn lc als EC gl fs Mem0,
+  wf_State (NDopsem.mkState S TD Ps
+              ((NDopsem.mkEC F B (c::cs) tmn lc als)::EC) gl fs Mem0) ->
+  wf_lc lc.
+Proof.
+  intros. destruct TD.
+  destruct H as 
+    [Hwfg [HwfSystem [HmInS [
+     [Hreach1 [HBinF1 [HFinPs1 [Hwflc1 [Hinscope1 [l3 [ps3 [cs3' Heq1]]]]]]]] 
+     [HwfEC HwfCall]]]]
+    ]; auto.
+Qed.  
+
+Tactic Notation "sInsn_cases" tactic(first) tactic(c) :=
+  first;
+  [ c "sReturn" | c "sReturnVoid" | c "sBranch" | c "sBranch_uncond" |
+    c "sBop" | (* c "sFBop" | c "sExtractValue" | c "sInsertValue" |*)
+    c "sMalloc" | c "sFree" |
+    c "sAlloca" | c "sLoad" | c "sStore" | c "sGEP" |
+    (*c "sTrunc" | c "sExt" | *)
+    c "sCast" | 
+    (*c "sIcmp" | c "sFcmp" | c "sSelect" |  *)
+    c "sCall" (*| c "sExCall"*) ].
+
+Lemma lookupFdefViaPtr_inversion : forall Ps fs fptr f,
+  lookupFdefViaPtr Ps fs fptr = Some f ->
+  exists fn,
+    lookupFdefViaGVFromFunTable fs fptr = Some fn /\
+    lookupFdefViaIDFromProducts Ps fn = Some f.
+Admitted.
+
+Lemma preservation : forall S1 S2 tr,
+  sInsn S1 S2 tr -> wf_State S1 -> wf_State S2.
+Proof.
+  intros S1 S2 tr HdsInsn HwfS1.
+  (sInsn_cases (induction HdsInsn) Case); destruct TD as [los nts].
+Focus.
+Case "sReturn".
+  destruct HwfS1 as 
+    [Hwfg [HwfSystem [HmInS [
+     [Hreach1 [HBinF1 [HFinPs1 [Hwflc1 [Hinscope1 [l1 [ps1 [cs1' Heq1]]]]]]]] 
+     [
+       [
+         [Hreach2 [HBinF2 [HFinPs2 [Hwflc2 [Hinscope2 [l2 [ps2 [cs2' Heq2]]]]]]]]
+         [HwfEC HwfCall]
+       ]
+       HwfCall'
+     ]
+    ]]]]; subst.
+  remember (inscope_of_cmd F' (block_intro l2 ps2 (cs2' ++ c' :: cs') tmn') c')
+    as R2.
+  destruct R2; try solve [inversion Hinscope2].
+  remember (inscope_of_tmn F
+             (block_intro l1 ps1 (cs1' ++ nil)(insn_return rid RetTy Result))
+             (insn_return rid RetTy Result)) as R1. 
+  destruct R1; try solve [inversion Hinscope1].
+  split; auto.
+  split; auto.
+  SCase "1".
+    split; auto.
+    split; auto.  
+    split; auto. 
+    split; auto.
+    split; auto.
+    split. eapply returnUpdateLocals__wf_lc in H1; eauto.
+    split.
+    SSCase "1.1".
+      destruct cs'; simpl_env in *.
+      SSSCase "1.1.1".
+        assert (~ In (getCmdLoc c') (getCmdsLocs cs2')) as Hnotin.
+          eapply wf_system__uniq_block with (f:=F') in HwfSystem; eauto.        
+          simpl in HwfSystem.
+          apply NoDup_inv in HwfSystem.
+          destruct HwfSystem as [_ J].
+          apply NoDup_inv in J.
+          destruct J as [J _].
+          rewrite getCmdsLocs_app in J.
+          simpl in J.
+          apply NoDup_last_inv in J. auto.
+        apply inscope_of_cmd_tmn in HeqR2; auto.
+        destruct HeqR2 as [ids2 [J1 J2]].        
+        rewrite <- J1.
+        remember (getCmdID c') as R.
+        destruct c'; try solve [inversion H].
+        unfold NDopsem.returnUpdateLocals in H1. simpl in H1.
+        remember (NDopsem.getOperandValue (los,nts) Result lc gl) as R1.
+        destruct R1; try solve [inv H1].
+        destruct R.
+          destruct n; inv HeqR. inv H1.
+          assert (Hwfc := HBinF2).
+          assert (In (insn_call i0 false c t v p) 
+            (cs2'++[insn_call i0 false c t v p])) as HinCs.
+            apply in_or_app. right. simpl. auto.
+          eapply wf_system__wf_cmd with (c:=insn_call i0 false c t v p) 
+            in Hwfc; eauto.
+          inv Hwfc.
+          eapply wf_defs_updateAddAL with (t1:=typ1);
+            eauto using getOperandValue__inhabited.
+            eapply uniqF__lookupTypViaIDFromFdef; eauto.
+              eapply wf_system__uniqFdef; eauto.
+
+          destruct n; inv HeqR. inv H1.
+          eapply wf_defs_eq; eauto. 
+        
+      SSSCase "1.1.2".
+        assert (NoDup (getCmdsLocs (cs2' ++ [c'] ++ [c] ++ cs'))) as Hnodup.
+          eapply wf_system__uniq_block with (f:=F') in HwfSystem; eauto.        
+          simpl in HwfSystem.
+          apply NoDup_inv in HwfSystem.
+          destruct HwfSystem as [_ J].
+          apply NoDup_inv in J.
+          destruct J as [J _]. auto.
+        apply inscope_of_cmd_cmd in HeqR2; auto.
+        destruct HeqR2 as [ids2 [J1 J2]].        
+        rewrite <- J1.
+        remember (getCmdID c') as R.
+        destruct c'; try solve [inversion H].
+        unfold NDopsem.returnUpdateLocals in H1. simpl in H1.
+        remember (NDopsem.getOperandValue (los,nts) Result lc gl) as R1.
+        destruct R1; try solve [inv H1].
+        destruct R.
+          destruct n; inv HeqR. inv H1.
+          assert (In (insn_call i0 false c0 t v p) 
+            (cs2'++[insn_call i0 false c0 t v p] ++ [c] ++ cs')) as HinCs.
+            apply in_or_app. right. simpl. auto.
+          assert (Hwfc := HBinF2).
+          eapply wf_system__wf_cmd with (c:=insn_call i0 false c0 t v p) 
+            in Hwfc; eauto.
+          inv Hwfc.
+          eapply wf_defs_updateAddAL with (t1:=typ1); 
+            eauto using getOperandValue__inhabited.
+            eapply uniqF__lookupTypViaIDFromFdef; eauto.
+              eapply wf_system__uniqFdef; eauto.
+
+          destruct n; inv HeqR. inv H1.
+          eapply wf_defs_eq; eauto. 
+    SSCase "1.2".
+      exists l2. exists ps2. exists (cs2'++[c']).   
+      simpl_env. auto.
+Unfocus.
+
+Focus.
+Case "sReturnVoid".
+  destruct HwfS1 as 
+    [Hwfg [HwfSystem [HmInS [
+     [Hreach1 [HBinF1 [HFinPs1 [Hwflc1 [Hinscope1 [l1 [ps1 [cs1' Heq1]]]]]]]] 
+     [
+       [
+         [Hreach2 [HBinF2 [HFinPs2 [Hwflc2 [Hinscope2 [l2 [ps2 [cs2' Heq2]]]]]]]]
+         [HwfEC HwfCall]
+       ]
+       HwfCall'
+     ]
+    ]]]]; subst.
+  remember (inscope_of_cmd F' (block_intro l2 ps2 (cs2' ++ c' :: cs') tmn') c')
+    as R2.
+  destruct R2; try solve [inversion Hinscope2].
+  remember (inscope_of_tmn F
+             (block_intro l1 ps1 (cs1' ++ nil)(insn_return_void rid))
+             (insn_return_void rid)) as R1. 
+  destruct R1; try solve [inversion Hinscope1].
+  split; auto.
+  split; auto.
+  SCase "1".
+    split; auto.
+    split; auto.
+    split; auto.
+    split; auto.
+    split; auto.
+    split; auto.
+    split.   
+    SSCase "1.1".
+      apply HwfCall' in HBinF1. simpl in HBinF1.
+      destruct cs'; simpl_env in *.
+      SSSCase "1.1.1".
+        assert (~ In (getCmdLoc c') (getCmdsLocs cs2')) as Hnotin.
+          eapply wf_system__uniq_block with (f:=F') in HwfSystem; eauto.        
+          simpl in HwfSystem.
+          apply NoDup_inv in HwfSystem.
+          destruct HwfSystem as [_ J].
+          apply NoDup_inv in J.
+          destruct J as [J _].
+          rewrite getCmdsLocs_app in J.
+          simpl in J.
+          apply NoDup_last_inv in J. auto.
+        clear - HeqR2 Hinscope2 H HwfCall' HBinF1 Hnotin H1.
+        apply inscope_of_cmd_tmn in HeqR2; auto.
+        destruct HeqR2 as [ids2 [J1 J2]].        
+        rewrite <- J1.
+        remember (getCmdID c') as R.
+        destruct c'; try solve [inversion H].
+        destruct n; inversion H1.
+        simpl in HeqR. subst R.
+        eapply wf_defs_eq; eauto. 
+        
+      SSSCase "1.1.2".
+        assert (NoDup (getCmdsLocs (cs2' ++ [c'] ++ [c] ++ cs'))) as Hnodup.
+          eapply wf_system__uniq_block with (f:=F') in HwfSystem; eauto.        
+          simpl in HwfSystem.
+          apply NoDup_inv in HwfSystem.
+          destruct HwfSystem as [_ J].
+          apply NoDup_inv in J.
+          destruct J as [J _]. auto.
+        clear - HeqR2 Hinscope2 H HwfCall' HBinF1 Hnodup H1.
+        apply inscope_of_cmd_cmd in HeqR2; auto.
+        destruct HeqR2 as [ids2 [J1 J2]].        
+        rewrite <- J1.
+        remember (getCmdID c') as R.
+        destruct c'; try solve [inversion H].
+        destruct n; inversion H1.
+        simpl in HeqR. subst R.
+        eapply wf_defs_eq; eauto. 
+
+    SSCase "1.2".
+      exists l2. exists ps2. exists (cs2'++[c']).   
+      simpl_env. auto.
+Unfocus.
+
+Focus.
+Case "sBranch".
+  destruct HwfS1 as 
+    [Hwfg [HwfSystem [HmInS [
+     [Hreach1 [HBinF1 [HFinPs1 [Hwflc1 [Hinscope1 [l3 [ps3 [cs3' Heq1]]]]]]]]
+     [HwfEC HwfCall]]]]
+    ]; subst.
+  remember (inscope_of_tmn F
+             (block_intro l3 ps3 (cs3' ++ nil)(insn_br bid Cond l1 l2))
+             (insn_br bid Cond l1 l2)) as R1. 
+  destruct R1; try solve [inversion Hinscope1].
+  split; auto.
+  split; auto.
+  split; auto.
+  split; auto.
+  SCase "1".
+    split.
+      clear - Hreach1 H1 HBinF1 HFinPs1 HmInS HwfSystem.
+      eapply wf_system__uniqFdef in HwfSystem; eauto.
+      unfold isReachableFromEntry in *.
+      destruct (isGVZero (los, nts) c).
+        symmetry in H1.
+        apply lookupBlockViaLabelFromFdef_inv in H1; eauto.
+        destruct H1 as [H1 _].
+        eapply reachable_successors; eauto.
+          simpl. auto.
+      
+        symmetry in H1.
+        apply lookupBlockViaLabelFromFdef_inv in H1; eauto.
+        destruct H1 as [H1 _].
+        eapply reachable_successors; eauto.
+          simpl. auto.
+    split. 
+      clear - H1 HBinF1 HFinPs1 HmInS HwfSystem.
+      eapply wf_system__uniqFdef with (f:=F) in HwfSystem; eauto.
+      destruct (isGVZero (los, nts) c).
+        symmetry in H1.
+        apply lookupBlockViaLabelFromFdef_inv in H1; auto.
+          destruct H1; auto.
+        symmetry in H1.
+        apply lookupBlockViaLabelFromFdef_inv in H1; auto.
+          destruct H1; auto.
+    split; auto.
+    split. apply wf_lc_br_aux in H2; auto.
+    split.
+      assert (HwfF := HwfSystem).
+      eapply wf_system__wf_fdef with (f:=F) in HwfF; eauto.
+      eapply wf_system__uniqFdef with (f:=F) in HwfSystem; eauto.
+      clear - H0 HeqR1 H1 Hinscope1 H2 HwfSystem HBinF1 HwfF Hwflc1.
+      eapply inscope_of_tmn_br in HeqR1; eauto.
+      destruct HeqR1 as [ids0' [HeqR1 [J1 J2]]].
+      destruct cs'; rewrite <- HeqR1; auto.
+
+      exists l'. exists ps'. exists nil. simpl_env. auto.
+Unfocus.
+
+Focus.
+Case "sBranch_uncond".
+  destruct HwfS1 as 
+    [Hwfg [HwfSystem [HmInS [
+     [Hreach1 [HBinF1 [HFinPs1 [Hwflc1 [Hinscope1 [l3 [ps3 [cs3' Heq1]]]]]]]] 
+     [HwfEC HwfCall]]]]
+    ]; subst.
+  remember (inscope_of_tmn F
+             (block_intro l3 ps3 (cs3' ++ nil)(insn_br_uncond bid l0))
+             (insn_br_uncond bid l0)) as R1. 
+  destruct R1; try solve [inversion Hinscope1].
+  split; auto.
+  split; auto.
+  split; auto.
+  SCase "1".
+    split; auto.
+    split.
+      clear - Hreach1 H HBinF1 HFinPs1 HmInS HwfSystem.
+      eapply wf_system__uniqFdef with (f:=F) in HwfSystem; eauto.
+      unfold isReachableFromEntry in *.
+      symmetry in H.
+      apply lookupBlockViaLabelFromFdef_inv in H; auto.
+      destruct H as [H _].
+      eapply reachable_successors; eauto.
+        simpl. auto.
+    split.
+      clear - H HBinF1 HFinPs1 HmInS HwfSystem.
+      eapply wf_system__uniqFdef with (f:=F) in HwfSystem; eauto.
+      symmetry in H.
+      apply lookupBlockViaLabelFromFdef_inv in H; auto.
+        destruct H; auto.
+    split; auto.
+    split. apply wf_lc_br_aux in H0; auto.
+    split.
+      assert (HwfF := HwfSystem).
+      eapply wf_system__wf_fdef with (f:=F) in HwfF; eauto.
+      eapply wf_system__uniqFdef with (f:=F) in HwfSystem; eauto.
+      clear - H0 HeqR1 Hinscope1 H HwfSystem HBinF1 HwfF Hwflc1.
+      assert (Hwds := HeqR1).
+      eapply inscope_of_tmn_br_uncond with (cs':=cs')(l':=l')(ps':=ps')
+        (tmn':=tmn') in HeqR1; eauto.
+      destruct HeqR1 as [ids0' [HeqR1 [J1 J2]]].
+      destruct cs'; rewrite <- HeqR1; auto.
+
+      exists l'. exists ps'. exists nil. simpl_env. auto.
+Unfocus.
+
+Case "sBop". eapply preservation_cmd_updated_case in HwfS1; simpl; eauto.
+  eapply BOP__inhabited; eauto using wf_State__wf_lc.
+(*
+Case "dsFBop". eapply preservation_cmd_updated_case in HwfS1; simpl; eauto.
+Case "dsExtractValue".
+  assert (exists t0, getSubTypFromConstIdxs idxs t = Some t0) as J.
+    destruct HwfS1 as 
+      [Hwfg [HwfSystem [HmInS [
+         [Hreach1 [HBinF1 [HFinPs1 [Hinscope1 [l3 [ps3 [cs3' Heq1]]]]]]] 
+         [HwfEC HwfCall]]]]
+      ]; subst.
+    eapply wf_system__wf_cmd with (c:=insn_extractvalue id0 t v idxs) in HBinF1; 
+      eauto.
+      inv HBinF1; eauto.
+      apply in_or_app; simpl; auto.
+
+  destruct J as [t0 J].
+  eapply preservation_cmd_updated_case in HwfS1; simpl; eauto.
+Case "dsInsertValue". 
+  eapply preservation_cmd_updated_case in HwfS1; simpl; eauto.
+*)
+Case "sMalloc". eapply preservation_cmd_updated_case in HwfS1; simpl; eauto.
+  apply singleton_inhabited.
+Case "sFree". eapply preservation_cmd_non_updated_case in HwfS1; eauto.
+Case "sAlloca". eapply preservation_cmd_updated_case in HwfS1; simpl; eauto.
+  apply singleton_inhabited.
+Case "sLoad".  eapply preservation_cmd_updated_case in HwfS1; simpl; eauto.
+  apply gv2gvs__inhabited.
+Case "sStore". eapply preservation_cmd_non_updated_case in HwfS1; eauto.
+Case "sGEP". 
+  assert (J:=HwfS1).
+  destruct J as 
+    [Hwfg [HwfSystem [HmInS [
+         [Hreach1 [HBinF1 [HFinPs1 [Hwflc1 [Hinscope1 [l3 [ps3 [cs3' Heq1]]]]]]]]
+         [HwfEC HwfCall]]]]
+    ]; subst.
+  assert (exists t0, getGEPTyp idxs t = Some t0) as J.
+    eapply wf_system__wf_cmd with (c:=insn_gep id0 inbounds0 t v idxs) in HBinF1;
+      eauto.
+      inv HBinF1; eauto.
+      apply in_or_app; simpl; auto.
+  destruct J as [t0 J].
+  eapply preservation_cmd_updated_case in HwfS1; simpl; eauto.
+    apply getOperandValue__inhabited in H; auto.
+    apply values2GVs__inhabited in H0; auto.
+    destruct H0 as [vidxs0 H0].
+    eapply GEP__inhabited in H1; eauto. 
+
+(*
+Case "dsTrunc". eapply preservation_cmd_updated_case in HwfS1; simpl; eauto.
+Case "dsExt". eapply preservation_cmd_updated_case in HwfS1; simpl; eauto.
+*)
+Case "sCast". eapply preservation_cmd_updated_case in HwfS1; simpl; eauto.
+  eapply CAST__inhabited; eauto using wf_State__wf_lc.
+(*
+Case "dsIcmp". eapply preservation_cmd_updated_case in HwfS1; simpl; eauto.
+Case "dsFcmp". eapply preservation_cmd_updated_case in HwfS1; simpl; eauto.
+Case "dsSelect".
+  destruct (isGVZero (los, nts) c); 
+  eapply preservation_cmd_updated_case in HwfS1; simpl; eauto.
+*)
+Focus.
+Case "sCall".
+  destruct HwfS1 as [Hwfg [HwfSys [HmInS [
+    [Hreach [HBinF [HFinPs [Hwflc [Hinscope [l1 [ps [cs'' Heq]]]]]]]]
+    [HwfECs HwfCall]]]]]; subst.
+  assert (InProductsB (product_fdef (fdef_intro 
+    (fheader_intro fa rt fid la va) lb)) Ps = true) as HFinPs'.
+    apply lookupFdefViaPtr_inversion in H1.
+    destruct H1 as [fn [H11 H12]].
+    eapply lookupFdefViaIDFromProducts_inv; eauto.
+  split; auto.
+  split; auto.
+  split; auto.
+  split.
+  SCase "1".     
+    assert (forall gv : GVs, In gv gvs -> Ensembles.Inhabited GenericValue gv)
+      as JJ.
+      eapply params2GVs_inhabited; eauto.
+    split.
+      simpl. eapply reachable_entrypoint; eauto.
+    split.
+     apply entryBlockInFdef in H2; auto.
+    split; auto.
+    split.
+     apply initLocals__wf_lc; eauto.
+    split.
+     assert (ps'=nil) as EQ.
+       eapply entryBlock_has_no_phinodes with (ifs:=nil)(s:=S); eauto.        
+     subst.
+     apply dom_entrypoint in H2.
+     destruct cs'.
+       unfold inscope_of_tmn.
+       remember ((dom_analyze (fdef_intro (fheader_intro fa rt fid la va) lb)) 
+         !! l') as R.
+       destruct R.
+       eapply preservation_dbCall_case; eauto.
+
+       unfold inscope_of_cmd.
+       remember ((dom_analyze (fdef_intro (fheader_intro fa rt fid la va) lb)) 
+         !! l') as R.
+       destruct R. simpl.
+       destruct (eq_atom_dec (getCmdLoc c) (getCmdLoc c)) as [|n]; 
+         try solve [contradict n; auto]. 
+       eapply preservation_dbCall_case; eauto.
+
+    exists l'. exists ps'. exists nil. simpl_env. auto.
+  split.
+  SCase "2".
+    repeat (split; auto). eauto.
+  SCase "3".
+    simpl. intros b HbInBs. destruct b.
+    destruct t; auto.
+
+Unfocus.
+
+(*
+Case "dsExCall". 
+  unfold exCallUpdateLocals in H2.
+  destruct noret0.
+    inv H2.
+
+    eapply preservation_cmd_non_updated_case in HwfS1; eauto.
+    destruct oresult; inv H2.
+    assert (exists t0, getCmdTyp (insn_call rid false ca ft fv lp) = Some t0)
+      as J.
+      destruct HwfS1 as 
+        [Hwfg [HwfSystem [HmInS [
+           [Hreach1 [HBinF1 [HFinPs1 [Hinscope1 [l3 [ps3 [cs3' Heq1]]]]]]] 
+           [HwfEC HwfCall]]]]
+        ]; subst.
+      eapply wf_system__wf_cmd with (c:=insn_call rid false ca ft fv lp) 
+        in HBinF1; eauto.
+      simpl.
+      inv HBinF1; eauto. 
+      apply in_or_app; simpl; auto.
+
+    destruct J as [t0 J].
+    eapply preservation_cmd_updated_case with (t0:=t0) in HwfS1; simpl; eauto.
+*)
+Qed.
+
+(*********************************************)
+(** * Progress *)
+
+Lemma state_tmn_typing : forall ifs s m f l1 ps1 cs1 tmn1 defs id1 lc,
+  isReachableFromEntry f (block_intro l1 ps1 cs1 tmn1) ->
+  wf_insn ifs s m f (block_intro l1 ps1 cs1 tmn1) (insn_terminator tmn1) ->
+  Some defs = inscope_of_tmn f (block_intro l1 ps1 cs1 tmn1) tmn1 ->
+  wf_defs f lc defs ->
+  uniqFdef f ->
+  In id1 (getInsnOperands (insn_terminator tmn1)) ->
+  exists t, exists gv, 
+    lookupTypViaIDFromFdef f id1 = munit t /\
+    lookupAL _ lc id1 = Some gv /\ wf_GVs gv t.
+Proof.
+  intros ifs s m f l1 ps1 cs1 tmn1 defs id1 lc Hreach HwfInstr Hinscope HwfDefs 
+    HuniqF HinOps.
+  apply wf_insn__wf_insn_base in HwfInstr; 
+    try solve [unfold isPhiNode; simpl; auto].
+  inv HwfInstr.  
+ 
+  assert (
+     In (f, block_intro l1 ps1 cs1 tmn1, insn_terminator tmn1, id1)
+     (unmake_list_fdef_block_insn_id
+        (make_list_fdef_block_insn_id
+           (map_list_id
+              (fun id_ : id =>
+               (f, block_intro l1 ps1 cs1 tmn1, insn_terminator tmn1, id_))
+              id_list)))
+    ) as G.
+    rewrite H5 in HinOps. clear - HinOps.
+    induction id_list; simpl in *; auto.
+      destruct HinOps as [HinOps | HinOps]; subst; auto.
+
+  apply wf_operand_list__elim with (f1:=f)(b1:=block_intro l1 ps1 cs1 tmn1)
+    (insn1:=insn_terminator tmn1)(id1:=id1) in H6; auto.
+
+  inv H6.
+  clear - H11 HwfDefs Hinscope H0 Hreach H9 HuniqF.
+  eapply wf_defs_elim; eauto.
+    unfold inscope_of_tmn in Hinscope.
+    destruct f. destruct f.
+    remember ((dom_analyze (fdef_intro (fheader_intro f t i0 a v) b)) !! l1) 
+      as R.
+    destruct R.  
+    symmetry in Hinscope.  
+    apply fold_left__spec in Hinscope.
+    destruct H11 as [J' | [J' | J']]; try solve [contradict J'; auto].
+      destruct Hinscope as [Hinscope _].
+      apply Hinscope.
+      destruct J' as [J' _].
+      destruct J' as [[cs2 [c1 [cs3 [J1 J2]]]] | [ps2 [p1 [ps3 [J1 J2]]]]]; 
+        subst.
+        rewrite getCmdsIDs_app. simpl. rewrite J2.
+        apply in_or_app. right.
+        apply in_or_app. left.
+        apply in_or_app. right. simpl. auto.
+    
+        rewrite getPhiNodesIDs_app. simpl.
+        apply in_or_app. left. 
+        apply in_or_app. right. simpl. auto.
+          
+     unfold blockStrictDominates in J'.
+     rewrite <- HeqR in J'.
+     destruct block'.
+     assert (In l0 (ListSet.set_diff eq_atom_dec bs_contents [l1])) as J.       
+       destruct J' as [J1 J2].
+       apply ListSet.set_diff_intro; auto.
+         simpl. intro J. destruct J as [J | J]; auto.
+     destruct Hinscope as [_ [Hinscope _]].
+     assert (
+       lookupBlockViaLabelFromFdef (fdef_intro (fheader_intro f t i0 a v) b) l0 =
+       ret block_intro l0 p c t0) as J1.
+       apply blockInFdefB_lookupBlockViaLabelFromFdef; auto.
+         eapply lookupBlockViaIDFromFdef__blockInFdefB; eauto. 
+     apply Hinscope with (b1:=block_intro l0 p c t0) in J; auto.
+       apply J.
+       eapply lookupBlockViaIDFromFdef__InGetBlockIDs; eauto.
+Qed.
+
+Lemma state_cmd_typing : forall ifs s m f b c defs id1 lc,
+  NoDup (getBlockLocs b) ->
+  isReachableFromEntry f b ->
+  wf_insn ifs s m f b (insn_cmd c) ->
+  Some defs = inscope_of_cmd f b c ->
+  wf_defs f lc defs ->
+  uniqFdef f ->
+  In id1 (getInsnOperands (insn_cmd c)) ->
+  exists t, exists gv, 
+    lookupTypViaIDFromFdef f id1 = munit t /\
+    lookupAL _ lc id1 = Some gv /\ wf_GVs gv t.
+Proof.
+  intros ifs s m f b c defs id1 lc Hnodup Hreach HwfInstr Hinscope HwfDefs 
+    HuniqF HinOps.
+  apply wf_insn__wf_insn_base in HwfInstr;
+    try solve [unfold isPhiNode; simpl; auto].
+  inv HwfInstr.  
+
+  assert (
+     In (f, b, insn_cmd c, id1)
+     (unmake_list_fdef_block_insn_id
+        (make_list_fdef_block_insn_id
+           (map_list_id
+              (fun id_ : id =>
+               (f, b, insn_cmd c, id_))
+              id_list)))
+    ) as G.
+    rewrite H5 in HinOps. clear - HinOps.
+    induction id_list; simpl in *; auto.
+      destruct HinOps as [HinOps | HinOps]; subst; auto.
+
+  apply wf_operand_list__elim with (f1:=f)(b1:=b)(insn1:=insn_cmd c)(id1:=id1) 
+    in H6; auto.
+
+  inv H6. 
+  eapply wf_defs_elim; eauto.
+    unfold inscope_of_cmd in Hinscope.
+    destruct b. destruct f. destruct f.
+    remember ((dom_analyze (fdef_intro (fheader_intro f t0 i0 a v) b)) !! l0) 
+      as R.
+    destruct R.  
+    symmetry in Hinscope.  
+    apply fold_left__spec in Hinscope.
+    destruct H11 as [J' | [J' | J']]; try solve [contradict J'; auto].
+      destruct Hinscope as [Hinscope _].
+      apply Hinscope.
+      simpl in J'.
+      destruct J' as [[ps2 [p1 [ps3 [J1 J2]]]] | [cs1 [c1 [cs2 [cs3 [J1 J2]]]]]];
+        subst.
+
+        rewrite getPhiNodesIDs_app. simpl.
+        apply in_or_app. left. 
+        apply in_or_app. right. simpl. auto.
+          
+        clear - J2 Hnodup.
+        apply in_or_app. right.
+        apply in_or_app. left. 
+          simpl in Hnodup. apply NoDup_inv in Hnodup.
+          destruct Hnodup as [_ Hnodup].
+          apply NoDup_inv in Hnodup.
+          destruct Hnodup as [Hnodup _].
+          rewrite_env ((cs1 ++ c1 :: cs2) ++ c :: cs3).
+          rewrite_env ((cs1 ++ c1 :: cs2) ++ c :: cs3) in Hnodup.
+          apply NoDup__In_cmds_dominates_cmd; auto.
+            rewrite getCmdsIDs_app.
+            apply in_or_app. right. simpl. rewrite J2. simpl. auto.
+    
+     clear Hreach H0 HwfDefs.
+     unfold blockStrictDominates in J'.
+     rewrite <- HeqR in J'.
+     destruct block'.
+     assert (In l1 (ListSet.set_diff eq_atom_dec bs_contents [l0])) as J.       
+       destruct J' as [J1 J2].
+       apply ListSet.set_diff_intro; auto.
+         simpl. intro J. destruct J as [J | J]; auto.
+     destruct Hinscope as [_ [Hinscope _]].
+     assert (
+       lookupBlockViaLabelFromFdef (fdef_intro (fheader_intro f t0 i0 a v) b) l1
+         = ret block_intro l1 p0 c1 t1) as J1.
+       apply blockInFdefB_lookupBlockViaLabelFromFdef; auto.
+         eapply lookupBlockViaIDFromFdef__blockInFdefB; eauto. 
+     apply Hinscope with (b1:=block_intro l1 p0 c1 t1) in J; auto.
+       apply J.
+       eapply lookupBlockViaIDFromFdef__InGetBlockIDs; eauto.
+Qed.
+
+Lemma ogvs_lift_some : forall ogv, 
+  (exists gv, ogv = Some gv) -> exists gvs : GVs, %ogv% = ret gvs.
+Proof.
+  intros.
+  destruct H; subst.
+  simpl. eauto.
+Qed. 
+
+Lemma getOperandValue_inCmdOps_isnt_stuck : forall
+  (s : system)
+  (los : layouts)
+  (nts : namedts)
+  (ps : list product)
+  (f : fdef)
+  (cs : list cmd)
+  (tmn : terminator)
+  (lc : GVsMap)
+  (gl : GVMap)
+  (Hwfg : wf_global s gl)
+  (HwfSys1 : wf_system nil s)
+  (HmInS1 : moduleInSystemB (module_intro los nts ps) s = true)
+  (HfInPs : InProductsB (product_fdef f) ps = true)
+  (l1 : l)
+  (ps1 : phinodes)
+  (cs1 : list cmd)
+  (c : cmd)
+  (Hreach : isReachableFromEntry f (block_intro l1 ps1 (cs1 ++ c :: cs) tmn))
+  (HbInF : blockInFdefB (block_intro l1 ps1 (cs1 ++ c :: cs) tmn) f = true)
+  (l0 : list atom)
+  (HeqR : ret l0 = inscope_of_cmd f (block_intro l1 ps1 (cs1 ++ c :: cs) tmn) c)
+  (Hinscope : wf_defs f lc l0)
+  (v : value)
+  (Hvincs : valueInCmdOperands v c),
+  exists gv : GVs, 
+    NDopsem.getOperandValue (los, nts) v lc gl = ret gv.
+Proof.
+  intros.
+  destruct v as [vid | vc]; simpl.
+    assert (exists t, exists gv, 
+                lookupTypViaIDFromFdef f vid = munit t /\
+                lookupAL _ lc vid = Some gv /\ 
+                wf_GVs gv t) as Hlkup.
+      eapply state_cmd_typing; eauto. 
+      eapply wf_system__uniq_block; eauto.
+      eapply wf_system__wf_cmd; eauto using In_middle.
+      eapply wf_system__uniqFdef; eauto.
+      apply valueInCmdOperands__InOps; auto.
+    destruct Hlkup as [gt [gv [Hlktyp [Hlkup Hwfgv]]]].
+    simpl.
+    rewrite Hlkup. eauto.
+
+    assert (In c (cs1++c::cs)) as H. 
+      apply in_or_app. simpl. auto.
+    eapply wf_system__wf_cmd with (c:=c) in HbInF; eauto.
+    eapply wf_cmd__wf_value with (v:=value_const vc) in HbInF; eauto.
+    destruct HbInF as [t Hwfc].
+    inv Hwfc. apply ogvs_lift_some.
+    eapply const2GV_isnt_stuck with (S:=s)(t:=t); eauto.
+Qed.
+
+Lemma getOperandValue_inTmnOperans_isnt_stuck : forall
+  (s : system)
+  (los : layouts)
+  (nts : namedts)
+  (ps : list product)
+  (f : fdef)
+  (tmn : terminator)
+  (lc : GVsMap)
+  (gl : GVMap)
+  (Hwfg : wf_global s gl)
+  (HwfSys1 : wf_system nil s)
+  (HmInS1 : moduleInSystemB (module_intro los nts ps) s = true)
+  (HfInPs : InProductsB (product_fdef f) ps = true)
+  (l1 : l)
+  (ps1 : phinodes)
+  (cs1 : list cmd)
+  (Hreach : isReachableFromEntry f (block_intro l1 ps1 cs1 tmn))
+  (HbInF : blockInFdefB (block_intro l1 ps1 cs1 tmn) f = true)
+  (l0 : list atom)
+  (HeqR : ret l0 = inscope_of_tmn f (block_intro l1 ps1 cs1 tmn) tmn)
+  (Hinscope : wf_defs f lc l0)
+  (v : value)
+  (Hvincs : valueInTmnOperands v tmn),
+  exists gv : GVs, NDopsem.getOperandValue (los, nts) v lc gl = ret gv.
+Proof.
+  intros.
+  destruct v as [vid | vc].
+    assert (HwfInstr:=HbInF).
+    eapply wf_system__wf_tmn in HwfInstr; eauto.
+    assert (exists t, exists gv, 
+      lookupTypViaIDFromFdef f vid = munit t /\
+      lookupAL _ lc vid = Some gv /\ 
+      wf_GVs gv t) as Hlkup.
+      eapply state_tmn_typing; eauto. 
+      eapply wf_system__uniqFdef; eauto.
+      apply valueInTmnOperands__InOps; auto.
+    destruct Hlkup as [gt [gv [Hlktyp [Hlkup Hwfgv]]]].
+    simpl.
+    rewrite Hlkup. eauto.
+
+    eapply wf_system__wf_tmn in HbInF; eauto.
+    eapply wf_tmn__wf_value with (v:=value_const vc) in HbInF; eauto.
+    destruct HbInF as [ct Hwfc].
+    inv Hwfc. apply ogvs_lift_some.
+    eapply const2GV_isnt_stuck with (S:=s)(t:=ct); eauto.
+Qed.
+
+Lemma values2GVs_isnt_stuck : forall
+  l22
+  (s : system)
+  los nts
+  (ps : list product)
+  (f : fdef)
+  (i0 : id)
+  (i1 : inbounds)
+  (t : typ)
+  (v : value)
+  (l2 : list_value)
+  (cs : list cmd)
+  (tmn : terminator)
+  (lc : GVsMap)
+  (gl : GVMap)
+  (Hwfg1 : wf_global s gl)
+  (HwfSys1 : wf_system nil s)
+  (HmInS1 : moduleInSystemB (module_intro los nts ps) s = true)
+  (HfInPs : InProductsB (product_fdef f) ps = true)
+  (l1 : l)
+  (ps1 : phinodes)
+  (cs1 : list cmd)
+  (Hreach : isReachableFromEntry f
+             (block_intro l1 ps1 (cs1 ++ insn_gep i0 i1 t v l2 :: cs) tmn))
+  (HbInF : blockInFdefB
+            (block_intro l1 ps1 (cs1 ++ insn_gep i0 i1 t v l2 :: cs) tmn) f =
+          true)
+  (l0 : list atom)
+  (HeqR : ret l0 =
+         inscope_of_cmd f
+           (block_intro l1 ps1 (cs1 ++ insn_gep i0 i1 t v l2 :: cs) tmn)
+           (insn_gep i0 i1 t v l2))
+  (Hinscope : wf_defs f lc l0)
+  (Hex : exists l21, l2 = app_list_value l21 l22),
+  exists vidxs, NDopsem.values2GVs (los, nts) l22 lc gl = Some vidxs.
+Proof.
+  induction l22; intros; simpl; eauto.
+    destruct Hex as [l21 Hex]; subst.
+    assert (exists gv, NDopsem.getOperandValue (los, nts) v lc gl = Some gv) 
+      as J.
+      eapply getOperandValue_inCmdOps_isnt_stuck; eauto.
+        simpl. unfold valueInListValue. right. 
+        apply in_app_list_value_right; simpl; auto.
+
+    destruct J as [gv J].
+    rewrite J.         
+    eapply IHl22 in HbInF; eauto.  
+      destruct HbInF as [vidxs HbInF].
+      rewrite HbInF. eauto.
+
+      exists (app_list_value l21 (Cons_list_value v Nil_list_value)).
+        rewrite cons_eq_app_list_value.
+        rewrite cons_eq_app_list_value.
+        apply app_list_value_assoc.
+Qed.
+
+Lemma wf_phinodes__getIncomingValuesForBlockFromPHINodes : forall
+  (s : system)
+  (los : layouts)
+  (nts : namedts)
+  (ps : list product)
+  (f : fdef)
+  l0
+  (lc : GVsMap)
+  (gl : GVMap)
+  (t : list atom)
+  l1 ps1 cs1 tmn1
+  (Hwfg : wf_global s gl)
+  (HeqR : ret t = inscope_of_tmn f (block_intro l1 ps1 cs1 tmn1) tmn1)
+  (Hinscope : wf_defs f lc t)
+  (HuniqF : uniqFdef f)
+  (ps' : phinodes)
+  (cs' : cmds)
+  (tmn' : terminator)
+  ps2
+  (Hreach : isReachableFromEntry f (block_intro l0 ps' cs' tmn'))
+  (HbInF : blockInFdefB
+            (block_intro l1 ps1 cs1 tmn1) f = true)
+  (HwfB : wf_block nil s (module_intro los nts ps) f 
+             (block_intro l1 ps1 cs1 tmn1))
+  (H8 : wf_phinodes nil s (module_intro los nts ps) f
+         (block_intro l0 ps' cs' tmn') ps2)
+  (Hsucc : In l0 (successors_terminator tmn1))
+  (Hin: exists ps1, ps' = ps1 ++ ps2),
+   exists RVs : list (id * GVs),
+     NDopsem.getIncomingValuesForBlockFromPHINodes (los, nts) ps2 
+       (block_intro l1 ps1 cs1 tmn1) gl lc =
+       ret RVs.
+Proof.
+  intros.
+  induction ps2; simpl.
+    exists nil. auto.
+  
+    destruct a. inv H8. inv H6.
+    assert (exists v, getValueViaLabelFromValuels l2 l1 = Some v) as J.      
+      clear - H14 HbInF HuniqF Hsucc.
+      inv H14.
+      unfold check_list_value_l in H0.
+      remember (split (unmake_list_value_l l2)) as R.
+      destruct R.
+      destruct H0 as [J1 [J2 J3]].
+      eapply In__getValueViaLabelFromValuels; eauto.
+      destruct J2 as [_ J2].
+      apply J2.
+      eapply successors_predOfBlock; eauto.
+
+    destruct J as [v J].
+    rewrite J.
+    destruct v as [vid | vc].
+    Case "vid".
+      assert (exists gv1, lookupAL _ lc vid = Some gv1) as J1.
+        Focus.
+        destruct H14 as [Hwfops Hwfvls].             
+        assert (Hnth:=J).
+        eapply getValueViaLabelFromValuels__nth_list_value_l in Hnth; eauto.
+        destruct Hnth as [n Hnth].
+        assert (HwfV:=J).
+        eapply wf_value_list__getValueViaLabelFromValuels__wf_value in HwfV; eauto.
+        eapply wf_phi_operands__elim in Hwfops; eauto.
+        destruct Hwfops as [Hneqid [vb [b1 [Hlkvb [Hlkb1 Hdom]]]]].
+        assert (b1 = block_intro l1 ps1 cs1 tmn1) 
+          as EQ.
+          clear - Hlkb1 HbInF HuniqF.
+          apply blockInFdefB_lookupBlockViaLabelFromFdef in HbInF; auto.
+          rewrite HbInF in Hlkb1. inv Hlkb1; auto.
+
+        subst.
+        clear - Hdom Hinscope HeqR J Hreach H2 HbInF Hlkvb Hlkb1 HuniqF.
+        destruct Hdom as [J3 | J3]; try solve [contradict Hreach; auto].
+        clear Hreach.        
+        unfold blockDominates in J3.         
+        destruct vb.
+        unfold inscope_of_tmn in HeqR.
+        destruct f. destruct f.
+        remember ((dom_analyze (fdef_intro (fheader_intro f t2 i0 a v) b)) !! l1)
+          as R1.
+        destruct R1.
+        symmetry in HeqR.    
+        apply fold_left__spec in HeqR.
+        destruct (eq_atom_dec l3 l1); subst.
+        SCase "l3=l1".
+          destruct HeqR as [HeqR _].
+          assert (In vid t) as G.
+            clear - J HeqR Hlkb1 J3 Hlkvb HbInF HuniqF.
+            assert (J':=Hlkvb).
+            apply lookupBlockViaIDFromFdef__blockInFdefB in Hlkvb.
+            apply lookupBlockViaLabelFromFdef_inv in Hlkb1; auto.
+            destruct Hlkb1 as [J1 J2].
+            eapply blockInFdefB_uniq in J2; eauto.
+            destruct J2 as [J2 [J4 J5]]; subst.
+            apply lookupBlockViaIDFromFdef__InGetBlockIDs in J'.
+            simpl in J'.
+            apply HeqR.
+            rewrite_env ((getPhiNodesIDs ps1 ++ getCmdsIDs cs1)++getArgsIDs a).
+            apply in_or_app; auto.       
+          apply wf_defs_elim with (id1:=vid) in Hinscope; auto.
+          destruct Hinscope as [? [gv1 [? [Hinscope ?]]]].
+          exists gv1. auto.
+
+        SCase "l3<>l1".
+          assert (In l3 (ListSet.set_diff eq_atom_dec bs_contents [l1])) as G.
+            apply ListSet.set_diff_intro; auto.
+              simpl. intro JJ. destruct JJ as [JJ | JJ]; auto.
+          assert (
+            lookupBlockViaLabelFromFdef 
+              (fdef_intro (fheader_intro f t2 i0 a v) b) l3 = 
+              ret block_intro l3 p c t1) as J1.
+            clear - Hlkvb HuniqF.
+            apply lookupBlockViaIDFromFdef__blockInFdefB in Hlkvb.
+            apply blockInFdefB_lookupBlockViaLabelFromFdef in Hlkvb; auto.
+          destruct HeqR as [_ [HeqR _]].
+          apply HeqR in J1; auto.
+          assert (In vid t) as InVid.
+            clear - J1 HeqR Hlkb1 J3 Hlkvb HbInF HuniqF.
+            apply J1.
+            apply lookupBlockViaIDFromFdef__InGetBlockIDs in Hlkvb; auto.
+          apply wf_defs_elim with (id1:=vid) in Hinscope; auto.
+          destruct Hinscope as [? [gv1 [? [Hinscope ?]]]].
+          exists gv1. auto.
+        Unfocus.
+  
+      destruct J1 as [gv1 J1].
+      simpl. rewrite J1. 
+      apply IHps2 in H7.
+        destruct H7 as [RVs H7].
+        rewrite H7. 
+        exists ((i0, gv1) :: RVs). auto.
+  
+        destruct Hin as [ps3 Hin]. subst.
+        exists (ps3++[insn_phi i0 t0 l2]).
+        simpl_env. auto.
+  
+    Case "vc".
+      eapply wf_value_list__getValueViaLabelFromValuels__wf_value in H2; eauto.
+      inv H2.
+      destruct (@const2GV_isnt_stuck (los,nts) s gl vc t0); auto.
+      simpl. rewrite H.
+      apply IHps2 in H7.
+        destruct H7 as [RVs H7].
+        rewrite H7. simpl.
+        exists ((i0, $ x $) :: RVs). auto.
+  
+        destruct Hin as [ps3 Hin]. subst.
+        exists (ps3++[insn_phi i0 t0 l2]).
+        simpl_env. auto.
+Qed.
+
+Lemma params2GVs_isnt_stuck : forall
+  p22
+  (s : system)
+  los nts
+  (ps : list product)
+  (f : fdef)
+  (i0 : id)
+  n c t v p2
+  (cs : list cmd)
+  (tmn : terminator)
+  (lc : GVsMap)
+  (gl : GVMap)
+  (Hwfg1 : wf_global s gl)
+  (HwfSys1 : wf_system nil s)
+  (HmInS1 : moduleInSystemB (module_intro los nts ps) s = true)
+  (HfInPs : InProductsB (product_fdef f) ps = true)
+  (l1 : l)
+  (ps1 : phinodes)
+  (cs1 : list cmd)
+  (Hreach : isReachableFromEntry f
+             (block_intro l1 ps1 (cs1 ++ insn_call i0 n c t v p2 :: cs) tmn))
+  (HbInF : blockInFdefB
+            (block_intro l1 ps1 (cs1 ++ insn_call i0 n c t v p2 :: cs) tmn) f =
+          true)
+  (l0 : list atom)
+  (HeqR : ret l0 =
+         inscope_of_cmd f
+           (block_intro l1 ps1 (cs1 ++ insn_call i0 n c t v p2 :: cs) tmn)
+           (insn_call i0 n c t v p2))
+  (Hinscope : wf_defs f lc l0)
+  (Hex : exists p21, p2 = p21 ++ p22),
+  exists gvs, NDopsem.params2GVs (los, nts) p22 lc gl = Some gvs.
+Proof.
+  induction p22; intros; simpl; eauto.
+
+    destruct a.
+    destruct Hex as [p21 Hex]; subst.
+    assert (exists gv, NDopsem.getOperandValue (los, nts) v0 lc gl = Some gv)
+      as J.
+      eapply getOperandValue_inCmdOps_isnt_stuck; eauto.
+        simpl. unfold valueInParams. right. 
+        assert (J:=@in_split_r _ _ (p21 ++ (t0, v0) :: p22) (t0, v0)).
+        remember (split (p21 ++ (t0, v0) :: p22)) as R.
+        destruct R.
+        simpl in J. apply J.
+        apply In_middle.
+    destruct J as [gv J]. 
+    rewrite J.         
+    eapply IHp22 in HbInF; eauto.  
+      destruct HbInF as [vidxs HbInF].
+      rewrite HbInF. eauto.
+
+      exists (p21 ++ [(t0,v0)]). simpl_env. auto.
+Qed.
+
+Definition undefined_state (S : NDopsem.State): Prop :=
+  match S with
+  | {| NDopsem.CurTargetData := td;
+       NDopsem.ECS := {|
+                NDopsem.CurCmds := nil;
+                NDopsem.Terminator := insn_return _ _ _;
+                NDopsem.Allocas := als |} :: 
+              {| NDopsem.CurCmds := c::_ |} :: _;
+       NDopsem.Mem := M |} => free_allocas td M als = None
+  | _ => False
+  end \/
+  match S with
+  | {| NDopsem.CurTargetData := td;
+       NDopsem.ECS := {|
+                NDopsem.CurBB := _;
+                NDopsem.CurCmds := nil;
+                NDopsem.Terminator := insn_return_void _;
+                NDopsem.Allocas := als |} :: 
+              {| NDopsem.CurCmds := c::_ |} :: _;
+       NDopsem.Mem := M |} => free_allocas td M als = None \/ 
+                      match getCallerReturnID c with
+                      | Some _ => True
+                      | _ => False
+                      end
+  | _ => False
+  end \/
+  match S with
+  | {| NDopsem.ECS := {|
+                NDopsem.CurBB := block_intro _ _ _ (insn_unreachable _);
+                NDopsem.CurCmds := nil;
+                NDopsem.Terminator := (insn_unreachable _)
+               |} :: _
+     |} => True
+  | _ => False
+  end \/
+  match S with
+  | {| NDopsem.CurTargetData := td;
+       NDopsem.ECS := 
+         {| NDopsem.CurCmds := insn_malloc _ t v a::_ ; 
+            NDopsem.Locals := lc|} :: _;
+       NDopsem.Globals := gl;
+       NDopsem.Mem := M |}
+  | {| NDopsem.CurTargetData := td;
+       NDopsem.ECS := 
+         {| NDopsem.CurCmds := insn_alloca _ t v a::_ ; 
+            NDopsem.Locals := lc|} :: _;
+       NDopsem.Globals := gl;
+       NDopsem.Mem := M |} =>
+       match NDopsem.getOperandValue td v lc gl with
+       | Some gvs =>
+           match getTypeAllocSize td t with
+           | Some asz => ~ exists gv, exists M', exists mb, 
+               gv @ gvs /\ malloc td M asz gv a = Some (M', mb)
+           | _ => False
+           end
+       | _ => False
+       end
+  | _ => False
+  end \/
+  match S with
+  | {| NDopsem.CurTargetData := td;
+       NDopsem.ECS := {| NDopsem.CurCmds := insn_free _ _ v::_ ; 
+                             NDopsem.Locals := lc|} :: _;
+       NDopsem.Globals := gl;
+       NDopsem.Mem := M |} =>
+       match NDopsem.getOperandValue td v lc gl with
+       | Some gvs => ~ exists gv, exists M', gv @ gvs /\ free td M gv = Some M'
+       | _ => False
+       end
+  | _ => False
+  end \/
+  match S with
+  | {| NDopsem.CurTargetData := td;
+       NDopsem.ECS := {| NDopsem.CurCmds := insn_load _ t v a::_ ; 
+                             NDopsem.Locals := lc|} :: _;
+       NDopsem.Globals := gl;
+       NDopsem.Mem := M |} =>
+       match NDopsem.getOperandValue td v lc gl with
+       | Some gvs => 
+           ~ exists gv, exists gv', gv @ gvs /\ mload td M gv t a = Some gv'
+       | _ => False
+       end
+  | _ => False
+  end \/
+  match S with
+  | {| NDopsem.CurTargetData := td;
+       NDopsem.ECS := {| NDopsem.CurCmds := insn_store _ t v v0 a::_ ; 
+                             NDopsem.Locals := lc|} :: _;
+       NDopsem.Globals := gl;
+       NDopsem.Mem := M |} =>
+       match NDopsem.getOperandValue td v lc gl, 
+             NDopsem.getOperandValue td v0 lc gl with
+       | Some gvs, Some mgvs => 
+           ~ (exists gv, exists mgv, exists M', gv @ gvs /\ mgv @ mgvs /\ 
+                mstore td M mgv t gv a = Some M')
+       | _, _ => False
+       end
+  | _ => False
+  end \/
+  match S with
+  | {| NDopsem.CurTargetData := td;
+       NDopsem.CurProducts := ps;
+       NDopsem.ECS := {| NDopsem.CurCmds := insn_call i0 n _ _ v p::_ ; 
+                             NDopsem.Locals := lc|} :: _;
+       NDopsem.Globals := gl;
+       NDopsem.FunTable := fs;
+       NDopsem.Mem := M |} => 
+       match NDopsem.getOperandValue td v lc gl with
+       | Some fptrs =>
+           ~ (exists fptr, exists f, fptr @ fptrs /\ 
+                lookupFdefViaPtr ps fs fptr = Some f)
+       | _ => False
+       end
+(*
+             lookupExFdecViaGV td ps gl lc fs v with
+       | None, Some (fdec_intro (fheader_intro fa rt fid la va)) =>
+           match params2GVs td p lc gl with
+           | Some gvs =>
+             match callExternalFunction M fid gvs with
+             | Some (oresult, _) =>
+                match exCallUpdateLocals n i0 oresult lc with
+                | None => True
+                | _ => False
+                end
+             | None => True
+             end
+           | _ => False
+           end
+       | None, None => True
+       | _, _ => False
+       end
+*)
+  | _ => False
+  end.
+
+Ltac undefbehave := unfold undefined_state; simpl; 
+  try solve [
+    auto | 
+    right; auto | 
+    right; right; auto |  
+    right; right; right; right; auto |
+    right; right; right; right; right; auto |
+    right; right; right; right; right; right; auto |
+    right; right; right; right; right; right; right; auto |
+    right; right; right; right; right; right; right; right; auto
+  ].
+   
+Require Import Classical_Prop.
+
+Lemma progress : forall S1,
+  wf_State S1 -> 
+  s_isFinialState S1 = true \/ 
+  (exists S2, exists tr, sInsn S1 S2 tr) \/
+  undefined_state S1.
+Proof.
+  intros S1 HwfS1.
+  destruct S1 as [s [los nts] ps ecs gl fs M].
+  destruct HwfS1 as [Hwfg1 [HwfSys1 [HmInS1 HwfECs]]].
+  destruct ecs; try solve [inversion HwfECs].
+  destruct e as [f b cs tmn lc als].
+  destruct HwfECs as [[Hreach 
+                        [HbInF [HfInPs [Hwflc [Hinscope [l1 [ps1 [cs1 Heq]]]]]]]]
+                      [HwfECs HwfCall]].
+  subst b.
+  destruct cs.
+  Case "cs=nil".
+    remember (inscope_of_tmn f (block_intro l1 ps1 (cs1 ++ nil) tmn) tmn) as R.
+    destruct R; try solve [inversion Hinscope].
+    destruct tmn.
+    SCase "tmn=ret".
+      simpl in HwfCall.
+      destruct ecs.
+        simpl; auto.      
+
+        right.
+        destruct e as [f' b' cs' tmn' lc' als'].
+        assert (J:=HbInF).
+        apply HwfCall in J. clear HwfCall.
+        destruct cs'; try solve [inversion J].
+        destruct c; try solve [inversion J]. clear J.
+        remember (free_allocas (los,nts) M als) as Rm.
+        destruct Rm as [M' |]; try solve [undefbehave].
+        left. symmetry in HeqRm.
+        rename HeqRm into J.
+        assert (exists lc'', 
+          NDopsem.returnUpdateLocals (los,nts) (insn_call i1 n c t0 v0 p) v 
+            lc lc' gl = Some lc'') as Hretup.
+          unfold NDopsem.returnUpdateLocals. simpl.
+          assert (exists gv : GVs, 
+            NDopsem.getOperandValue (los, nts) v lc gl = ret gv) as H.
+            eapply getOperandValue_inTmnOperans_isnt_stuck; eauto.
+              simpl. auto.
+          destruct H as [gv H]. rewrite H.
+          destruct n.
+            exists lc'. auto.
+            exists (updateAddAL _ lc' i1 gv). auto.
+          
+        destruct Hretup as [lc'' Hretup].
+        exists (NDopsem.mkState s (los, nts) ps 
+                 ((NDopsem.mkEC f' b' cs' tmn' lc'' als')::ecs) gl fs M').
+        exists trace_nil.
+        eauto.  
+
+    SCase "tmn=ret void".
+      simpl in HwfCall.
+      destruct ecs.
+        simpl; auto.      
+
+        right.
+        destruct e as [f' b' cs' tmn' lc' als'].
+        assert (J:=HbInF).
+        apply HwfCall in J. clear HwfCall.
+        destruct cs'; try solve [inversion J].
+        destruct c; try solve [inversion J]. clear J.
+        remember (free_allocas (los,nts) M als) as Rm.
+        destruct Rm as [M' |]; try solve [undefbehave].
+        symmetry in HeqRm.
+        rename HeqRm into J.
+        destruct n; try solve [undefbehave].
+        left.
+        exists (NDopsem.mkState s (los, nts) ps 
+                 ((NDopsem.mkEC f' b' cs' tmn' lc' als')::ecs) gl fs M').
+        exists trace_nil.
+        eauto.  
+
+    SCase "tmn=br". 
+      right. left.
+      assert (uniqFdef f) as HuniqF.
+        eapply wf_system__uniqFdef; eauto.
+      assert (exists cond, NDopsem.getOperandValue (los,nts) v lc gl = 
+        Some cond) as Hget.
+        eapply getOperandValue_inTmnOperans_isnt_stuck; eauto.
+          simpl. auto.
+      destruct Hget as [cond Hget].
+      assert (exists c, c @ cond) as Hinh.
+        apply getOperandValue__inhabited in Hget; auto.
+        inv Hget. eauto.
+      destruct Hinh as [c Hinh].
+      assert (exists l', exists ps', exists cs', exists tmn',
+              Some (block_intro l' ps' cs' tmn') = 
+              (if isGVZero (los,nts) c
+                 then lookupBlockViaLabelFromFdef f l3
+                 else lookupBlockViaLabelFromFdef f l2)) as HlkB.
+        eapply wf_system__wf_tmn in HbInF; eauto.
+        inv HbInF. 
+        destruct block1 as [l2' ps2 cs2 tmn2].
+        destruct block2 as [l3' ps3 cs3 tmn3].
+        destruct (isGVZero (los, nts) c).
+          exists l3'. exists ps3. exists cs3. exists tmn3.
+          rewrite H11. auto.
+
+          exists l2'. exists ps2. exists cs2. exists tmn2.
+          rewrite H10. auto.
+
+      destruct HlkB as [l' [ps' [cs' [tmn' HlkB]]]].
+      assert (exists lc', NDopsem.switchToNewBasicBlock (los, nts) 
+        (block_intro l' ps' cs' tmn') 
+        (block_intro l1 ps1 (cs1++nil) (insn_br i0 v l2 l3)) gl lc = 
+          Some lc') as Hswitch.
+         assert (exists RVs, 
+           NDopsem.getIncomingValuesForBlockFromPHINodes (los, nts) ps'
+             (block_intro l1 ps1 (cs1++nil) (insn_br i0 v l2 l3)) gl lc =
+           Some RVs) as J.
+           assert (HwfB := HbInF).
+           eapply wf_system__blockInFdefB__wf_block in HwfB; eauto.
+           simpl_env in *.
+           destruct (isGVZero (los, nts) c).
+             assert (J:=HlkB).
+             symmetry in J.
+             apply lookupBlockViaLabelFromFdef_inv in J; auto.
+             destruct J as [Heq J]; subst.
+             eapply wf_system__lookup__wf_block in HlkB; eauto.
+             inv HlkB. clear H9 H10.
+             eapply wf_phinodes__getIncomingValuesForBlockFromPHINodes 
+               with (ps':=ps')(cs':=cs')(tmn':=tmn')(l0:=l'); eauto.
+               apply reachable_successors with (l0:=l1)(cs:=ps1)(ps:=cs1)
+                 (tmn:=insn_br i0 v l2 l'); simpl; auto.
+               simpl. auto.    
+               exists nil. auto.
+
+             assert (J:=HlkB).
+             symmetry in J.
+             apply lookupBlockViaLabelFromFdef_inv in J; auto.
+             destruct J as [Heq J]; subst.
+             eapply wf_system__lookup__wf_block in HlkB; eauto.
+             inv HlkB. clear H9 H10.
+             eapply wf_phinodes__getIncomingValuesForBlockFromPHINodes 
+               with (ps':=ps')(cs':=cs')(tmn':=tmn')(l0:=l'); eauto.
+               apply reachable_successors with (l0:=l1)(cs:=ps1)(ps:=cs1)
+                 (tmn:=insn_br i0 v l' l3); simpl; auto.
+               simpl. auto.    
+               exists nil. auto.
+         
+         destruct J as [RVs J].
+         unfold NDopsem.switchToNewBasicBlock. simpl.
+         rewrite J. 
+         exists (NDopsem.updateValuesForNewBlock RVs lc). auto.
+
+      destruct Hswitch as [lc' Hswitch].
+      exists (NDopsem.mkState s (los, nts) ps 
+              ((NDopsem.mkEC f (block_intro l' ps' cs' tmn') cs' tmn' lc' 
+              als)::ecs) gl fs M).
+      exists trace_nil. eauto.
+
+    SCase "tmn=br_uncond". 
+      right. left.
+      assert (uniqFdef f) as HuniqF.
+        eapply wf_system__uniqFdef; eauto.
+      assert (exists ps', exists cs', exists tmn',
+        Some (block_intro l2 ps' cs' tmn') = lookupBlockViaLabelFromFdef f l2) 
+          as HlkB.
+        eapply wf_system__wf_tmn in HbInF; eauto.
+        inv HbInF.        
+        exists ps1. exists (cs1++nil). exists (insn_br_uncond i0 l2).
+        rewrite H6. 
+        apply lookupBlockViaLabelFromFdef_inv in H6; auto.
+        destruct H6 as [H6 _]; subst. auto.
+
+      destruct HlkB as [ps' [cs' [tmn' HlkB]]].
+
+      assert (exists lc', NDopsem.switchToNewBasicBlock (los, nts) 
+        (block_intro l2 ps' cs' tmn') 
+        (block_intro l1 ps1 (cs1 ++ nil) (insn_br_uncond i0 l2)) gl lc = 
+          Some lc') as Hswitch.
+         assert (exists RVs, 
+           NDopsem.getIncomingValuesForBlockFromPHINodes (los, nts) ps'
+             (block_intro l1 ps1 (cs1 ++ nil) (insn_br_uncond i0 l2)) gl lc =
+           Some RVs) as J.
+           assert (HwfB := HbInF).
+           eapply wf_system__blockInFdefB__wf_block in HwfB; eauto.
+           eapply wf_system__lookup__wf_block in HlkB; eauto.
+           inv HlkB. clear H9 H10.
+           eapply wf_phinodes__getIncomingValuesForBlockFromPHINodes 
+             with (l0:=l2); eauto.      
+             apply reachable_successors with (l0:=l1)(cs:=ps1)(ps:=cs1++nil)
+               (tmn:=insn_br_uncond i0 l2); simpl; auto.
+             simpl. auto.
+             exists nil. auto.
+         
+         destruct J as [RVs J].
+         unfold NDopsem.switchToNewBasicBlock. simpl.
+         rewrite J. 
+         exists (NDopsem.updateValuesForNewBlock RVs lc). auto.
+
+      destruct Hswitch as [lc' Hswitch].
+      exists (NDopsem.mkState s (los, nts) ps 
+              ((NDopsem.mkEC f (block_intro l2 ps' cs' tmn') cs' tmn' lc' 
+              als)::ecs) gl fs M).
+      exists trace_nil. eauto.
+
+    SCase "tmn=unreachable".
+      undefbehave.
+
+  Case "cs<>nil".
+    assert (wf_insn nil s (module_intro los nts ps) f 
+      (block_intro l1 ps1 (cs1 ++ c :: cs) tmn) (insn_cmd c)) as Hwfc.
+      assert (In c (cs1++c::cs)) as H. 
+        apply in_or_app. simpl. auto.
+      eapply wf_system__wf_cmd with (c:=c) in HbInF; eauto.
+    remember (inscope_of_cmd f (block_intro l1 ps1 (cs1 ++ c :: cs) tmn) c) as R.
+    destruct R; try solve [inversion Hinscope].
+    right.
+    destruct c.
+  SCase "c=bop".
+    left.
+    assert (exists gv3, NDopsem.BOP (los,nts) lc gl b s0 v v0 = Some gv3) 
+      as Hinsn_bop.
+      unfold NDopsem.BOP.      
+      assert (exists gv, NDopsem.getOperandValue (los, nts) v lc gl = Some gv) 
+        as J.
+        eapply getOperandValue_inCmdOps_isnt_stuck; eauto.
+          simpl; auto.
+      assert (exists gv, NDopsem.getOperandValue (los, nts) v0 lc gl = Some gv) 
+        as J0.
+        eapply getOperandValue_inCmdOps_isnt_stuck; eauto.
+          simpl; auto.
+      destruct J as [gv J].
+      destruct J0 as [gv0 J0].
+      rewrite J. rewrite J0. 
+      eauto.
+    destruct Hinsn_bop as [gv3 Hinsn_bop].
+    exists 
+         {|
+         NDopsem.CurSystem := s;
+         NDopsem.CurTargetData := (los, nts);
+         NDopsem.CurProducts := ps;
+         NDopsem.ECS := {|
+                NDopsem.CurFunction := f;
+                NDopsem.CurBB := block_intro l1 ps1
+                           (cs1 ++ insn_bop i0 b s0 v v0 :: cs) tmn;
+                NDopsem.CurCmds := cs;
+                NDopsem.Terminator := tmn;
+                NDopsem.Locals := (updateAddAL _ lc i0 gv3);
+                NDopsem.Allocas := als |} :: ecs;
+         NDopsem.Globals := gl;
+         NDopsem.FunTable := fs;
+         NDopsem.Mem := M |}.
+     exists trace_nil. eauto.
+
+  SCase "c=fbop". admit.
+(*
+    left.
+    assert (exists gv3, FBOP (los,nts) lc gl f0 f1 v v0 = Some gv3) 
+      as Hinsn_fbop.
+      unfold FBOP.      
+      assert (exists gv, getOperandValue (los, nts) v lc gl = Some gv) as J.
+        eapply getOperandValue_inCmdOps_isnt_stuck; eauto.
+          simpl; auto.
+      assert (exists gv, getOperandValue (los, nts) v0 lc gl = Some gv) as J0.
+        eapply getOperandValue_inCmdOps_isnt_stuck; eauto.
+          simpl; auto.
+      destruct J as [gv J].
+      destruct J0 as [gv0 J0].
+      rewrite J. rewrite J0. 
+      unfold mfbop. 
+      destruct (GV2val (los, nts) gv); eauto.
+      destruct v1; eauto.
+      destruct (GV2val (los, nts) gv0); eauto.
+      destruct v1; eauto.
+      inv Hwfc.
+      apply wf_value__wf_typ in H7.
+      destruct H7 as [J1 J2].
+      destruct f1; try solve [eauto | inversion J1].
+
+    destruct Hinsn_fbop as [gv3 Hinsn_fbop].
+    exists 
+         {|
+         CurSystem := s;
+         CurTargetData := (los, nts);
+         CurProducts := ps;
+         ECS := {|
+                CurFunction := f;
+                CurBB := block_intro l1 ps1
+                           (cs1 ++ insn_fbop i0 f0 f1 v v0 :: cs) tmn;
+                CurCmds := cs;
+                Terminator := tmn;
+                Locals := (updateAddAL _ lc i0 gv3);
+                Allocas := als |} :: ecs;
+         Globals := gl;
+         FunTable := fs;
+         Mem := M |}.
+     exists trace_nil. eauto.
+*)
+  SCase "c=extractvalue". admit.
+(*
+    left.
+    assert (exists gv, getOperandValue (los, nts) v lc gl = Some gv) as J.
+      eapply getOperandValue_inCmdOps_isnt_stuck; eauto.
+        simpl; auto.
+    destruct J as [gv J].
+    assert (exists gv', extractGenericValue (los, nts) t gv l2 = Some gv') as J'.
+      unfold extractGenericValue.
+      destruct (intConsts2Nats (los, nts) l2); eauto.
+      destruct (mgetoffset (los, nts) t l3); eauto.
+      destruct (mget (los, nts) gv i1 t); eauto.
+    destruct J' as [gv' J'].
+    exists 
+         {|
+         CurSystem := s;
+         CurTargetData := (los, nts);
+         CurProducts := ps;
+         ECS := {|
+                CurFunction := f;
+                CurBB := block_intro l1 ps1
+                           (cs1 ++ insn_extractvalue i0 t v l2 :: cs) tmn;
+                CurCmds := cs;
+                Terminator := tmn;
+                Locals := (updateAddAL _ lc i0 gv');
+                Allocas := als |} :: ecs;
+         Globals := gl;
+         FunTable := fs;
+         Mem := M |}.
+     exists trace_nil. eauto.
+*)
+  SCase "c=insertvalue". admit.
+(*
+    left.
+    assert (exists gv, getOperandValue (los, nts) v lc gl = Some gv) as J.
+      eapply getOperandValue_inCmdOps_isnt_stuck; eauto.
+        simpl; auto.
+    destruct J as [gv J].
+    assert (exists gv', getOperandValue (los, nts) v0 lc gl = Some gv') as J'.
+      eapply getOperandValue_inCmdOps_isnt_stuck; eauto.
+        simpl; auto.
+    destruct J' as [gv' J'].
+    assert (exists gv'', insertGenericValue (los, nts) t gv l2 t0 gv' = 
+      Some gv'') as J''.
+      unfold insertGenericValue.
+      destruct (intConsts2Nats (los, nts) l2); eauto.
+      destruct (mgetoffset (los, nts) t l3); eauto.
+      destruct (mset (los, nts) gv i1 t0 gv'); eauto.
+    destruct J'' as [gv'' J''].
+    exists 
+         {|
+         CurSystem := s;
+         CurTargetData := (los, nts);
+         CurProducts := ps;
+         ECS := {|
+                CurFunction := f;
+                CurBB := block_intro l1 ps1
+                           (cs1 ++ insn_insertvalue i0 t v t0 v0 l2 :: cs) tmn;
+                CurCmds := cs;
+                Terminator := tmn;
+                Locals := (updateAddAL _ lc i0 gv'');
+                Allocas := als |} :: ecs;
+         Globals := gl;
+         FunTable := fs;
+         Mem := M |}.
+     exists trace_nil. eauto.
+*)
+
+  SCase "c=malloc". 
+    inv Hwfc. inv H12.
+    apply feasible_typ_inv in H.
+    destruct H as [ssz [asz [J1 J2]]].
+    assert (exists gvs, NDopsem.getOperandValue (los, nts) v lc gl = Some gvs) 
+      as J.
+      eapply getOperandValue_inCmdOps_isnt_stuck; eauto.
+        simpl; auto.
+    destruct J as [gvs J].
+    destruct (classic 
+      (exists gv, exists M', exists mb, 
+         gv @ gvs /\ malloc (los, nts) M asz gv a = Some (M', mb))) as 
+      [[gv [M' [mb [Hgvin Hex]]]] | Hnex].
+      left.
+      exists 
+         {|
+         NDopsem.CurSystem := s;
+         NDopsem.CurTargetData := (los, nts);
+         NDopsem.CurProducts := ps;
+         NDopsem.ECS := {|
+                NDopsem.CurFunction := f;
+                NDopsem.CurBB := block_intro l1 ps1
+                           (cs1 ++ insn_malloc i0 t v a :: cs) tmn;
+                NDopsem.CurCmds := cs;
+                NDopsem.Terminator := tmn;
+                NDopsem.Locals := 
+                  (updateAddAL _ lc i0 ($ (blk2GV (los, nts) mb) $));
+                NDopsem.Allocas := als |} :: ecs;
+         NDopsem.Globals := gl;
+         NDopsem.FunTable := fs;
+         NDopsem.Mem := M' |}.
+      exists trace_nil.
+      eauto.      
+      
+      unfold undefined_state.
+      right. rewrite J. rewrite J2. undefbehave.
+
+  SCase "free". 
+    assert (exists gvs, NDopsem.getOperandValue (los, nts) v lc gl = Some gvs) 
+      as J.
+      eapply getOperandValue_inCmdOps_isnt_stuck; eauto.
+        simpl; auto.
+    destruct J as [gvs J].
+    destruct (classic 
+      (exists gv, exists M', gv @ gvs /\ free (los, nts) M gv = Some M')) as 
+      [[gv [M' [Hgvin Hex]]] | Hnex].
+      left.
+      exists 
+         {|
+         NDopsem.CurSystem := s;
+         NDopsem.CurTargetData := (los, nts);
+         NDopsem.CurProducts := ps;
+         NDopsem.ECS := {|
+                NDopsem.CurFunction := f;
+                NDopsem.CurBB := block_intro l1 ps1
+                           (cs1 ++ insn_free i0 t v :: cs) tmn;
+                NDopsem.CurCmds := cs;
+                NDopsem.Terminator := tmn;
+                NDopsem.Locals := lc;
+                NDopsem.Allocas := als |} :: ecs;
+         NDopsem.Globals := gl;
+         NDopsem.FunTable := fs;
+         NDopsem.Mem := M' |}.
+      exists trace_nil.
+      eauto.      
+      
+      unfold undefined_state.
+      right. rewrite J. undefbehave.
+
+  SCase "alloca".
+    inv Hwfc. inv H12.
+    apply feasible_typ_inv in H.
+    destruct H as [ssz [asz [J1 J2]]].
+    assert (exists gvs, NDopsem.getOperandValue (los, nts) v lc gl = Some gvs) 
+      as J.
+      eapply getOperandValue_inCmdOps_isnt_stuck; eauto.
+        simpl; auto.
+    destruct J as [gvs J].
+    destruct (classic 
+      (exists gv, exists M', exists mb, 
+         gv @ gvs /\ malloc (los, nts) M asz gv a = Some (M', mb))) as 
+      [[gv [M' [mb [Hgvin Hex]]]] | Hnex].
+      left.
+      exists 
+         {|
+         NDopsem.CurSystem := s;
+         NDopsem.CurTargetData := (los, nts);
+         NDopsem.CurProducts := ps;
+         NDopsem.ECS := {|
+                NDopsem.CurFunction := f;
+                NDopsem.CurBB := block_intro l1 ps1
+                           (cs1 ++ insn_alloca i0 t v a :: cs) tmn;
+                NDopsem.CurCmds := cs;
+                NDopsem.Terminator := tmn;
+                NDopsem.Locals := 
+                  (updateAddAL _ lc i0 ($ (blk2GV (los, nts) mb) $));
+                NDopsem.Allocas := (mb::als) |} :: ecs;
+         NDopsem.Globals := gl;
+         NDopsem.FunTable := fs;
+         NDopsem.Mem := M' |}.
+      exists trace_nil.
+      eauto.      
+      
+      right.
+      unfold undefined_state.
+      right. rewrite J. rewrite J2. undefbehave.
+
+  SCase "load".
+    assert (exists gvs, NDopsem.getOperandValue (los, nts) v lc gl = Some gvs) 
+      as J.
+      eapply getOperandValue_inCmdOps_isnt_stuck; eauto.
+        simpl; auto.
+    destruct J as [gvs J].
+    destruct (classic 
+      (exists gv, exists gv', 
+      gv @ gvs /\ mload (los, nts) M gv t a = Some gv')) as 
+      [[gv [gv' [Hgvin Hex]]] | Hnex].
+      left.
+      exists 
+         {|
+         NDopsem.CurSystem := s;
+         NDopsem.CurTargetData := (los, nts);
+         NDopsem.CurProducts := ps;
+         NDopsem.ECS := {|
+                NDopsem.CurFunction := f;
+                NDopsem.CurBB := block_intro l1 ps1
+                           (cs1 ++ insn_load i0 t v a :: cs) tmn;
+                NDopsem.CurCmds := cs;
+                NDopsem.Terminator := tmn;
+                NDopsem.Locals := updateAddAL _ lc i0 ($ gv' $);
+                NDopsem.Allocas := als |} :: ecs;
+         NDopsem.Globals := gl;
+         NDopsem.FunTable := fs;
+         NDopsem.Mem := M |}.
+      exists trace_nil.
+      eauto.      
+
+      right.
+      unfold undefined_state.
+      right. rewrite J. undefbehave.
+      
+  SCase "store".
+    assert (exists gvs, NDopsem.getOperandValue (los, nts) v lc gl = Some gvs) 
+      as J.
+      eapply getOperandValue_inCmdOps_isnt_stuck; eauto.
+        simpl; auto.
+    destruct J as [gvs J].
+    assert (exists gvs, NDopsem.getOperandValue (los, nts) v0 lc gl = Some gvs) 
+      as J0.
+      eapply getOperandValue_inCmdOps_isnt_stuck; eauto.
+        simpl; auto.
+    destruct J0 as [mgvs J0].
+    destruct (classic (exists gv, exists mgv, exists M', 
+       gv @ gvs /\ mgv @ mgvs /\ mstore (los, nts) M mgv t gv a = Some M')) as
+      [[gv [mgv [M' [Hgvin [Hmgvin Hex]]]]] | Hnex].
+      left.
+      exists 
+         {|
+         NDopsem.CurSystem := s;
+         NDopsem.CurTargetData := (los, nts);
+         NDopsem.CurProducts := ps;
+         NDopsem.ECS := {|
+                NDopsem.CurFunction := f;
+                NDopsem.CurBB := block_intro l1 ps1
+                           (cs1 ++ insn_store i0 t v v0 a :: cs) tmn;
+                NDopsem.CurCmds := cs;
+                NDopsem.Terminator := tmn;
+                NDopsem.Locals := lc;
+                NDopsem.Allocas := als |} :: ecs;
+         NDopsem.Globals := gl;
+         NDopsem.FunTable := fs;
+         NDopsem.Mem := M' |}.
+      exists trace_nil.
+      eauto.      
+
+      right.
+      unfold undefined_state.
+      right. rewrite J. rewrite J0. undefbehave.
+
+  SCase "gep".
+    assert (exists gv, NDopsem.getOperandValue (los, nts) v lc gl = Some gv) 
+      as J.
+      eapply getOperandValue_inCmdOps_isnt_stuck; eauto.
+        simpl; auto.
+    destruct J as [mp J].
+    assert (exists vidxs, NDopsem.values2GVs (los, nts) l2 lc gl = Some vidxs) 
+      as J2.
+      eapply values2GVs_isnt_stuck; eauto.
+        exists Nil_list_value. auto.
+    destruct J2 as [vidxs J2].
+    assert (exists mp', NDopsem.GEP (los, nts) t mp vidxs i1 = Some mp') as J3.
+      unfold NDopsem.GEP. eauto.
+    destruct J3 as [mp' J3].
+    left.
+    exists 
+         {|
+         NDopsem.CurSystem := s;
+         NDopsem.CurTargetData := (los, nts);
+         NDopsem.CurProducts := ps;
+         NDopsem.ECS := {|
+                NDopsem.CurFunction := f;
+                NDopsem.CurBB := block_intro l1 ps1
+                           (cs1 ++ insn_gep i0 i1 t v l2 :: cs) tmn;
+                NDopsem.CurCmds := cs;
+                NDopsem.Terminator := tmn;
+                NDopsem.Locals := (updateAddAL _ lc i0 mp');
+                NDopsem.Allocas := als |} :: ecs;
+         NDopsem.Globals := gl;
+         NDopsem.FunTable := fs;
+         NDopsem.Mem := M |}.
+     exists trace_nil. eauto.
+
+  SCase "trunc". admit.
+(*
+    left.
+    assert (exists gv2, TRUNC (los,nts) lc gl t t0 v t1 = Some gv2) 
+      as Hinsn_trunc.
+      unfold TRUNC.      
+      assert (exists gv, getOperandValue (los, nts) v lc gl = Some gv) as J.
+        eapply getOperandValue_inCmdOps_isnt_stuck; eauto.
+          simpl; auto.
+      destruct J as [gv J].
+      rewrite J.
+      unfold mtrunc. 
+      destruct (GV2val (los, nts) gv); eauto.
+      inv Hwfc. 
+      inv H5; try solve [destruct v0; eauto].
+        rewrite H11.
+        destruct v0; eauto.
+          destruct floating_point2; try solve [eauto | inversion H13].
+    destruct Hinsn_trunc as [gv2 Hinsn_trunc].
+    exists 
+         {|
+         CurSystem := s;
+         CurTargetData := (los, nts);
+         CurProducts := ps;
+         ECS := {|
+                CurFunction := f;
+                CurBB := block_intro l1 ps1
+                           (cs1 ++ insn_trunc i0 t t0 v t1 :: cs) tmn;
+                CurCmds := cs;
+                Terminator := tmn;
+                Locals := (updateAddAL _ lc i0 gv2);
+                Allocas := als |} :: ecs;
+         Globals := gl;
+         FunTable := fs;
+         Mem := M |}.
+     exists trace_nil. eauto.
+*)
+  SCase "ext". admit.
+(*
+    left.
+    assert (exists gv2, EXT (los,nts) lc gl e t v t0 = Some gv2) 
+      as Hinsn_ext.
+      unfold EXT.      
+      assert (exists gv, getOperandValue (los, nts) v lc gl = Some gv) as J.
+        eapply getOperandValue_inCmdOps_isnt_stuck; eauto.
+          simpl; auto.
+      destruct J as [gv J].
+      rewrite J.
+      unfold mext. 
+      inv Hwfc. 
+      inv H5; try solve 
+        [destruct (GV2val (los, nts) gv); eauto; destruct v0; eauto].
+        rewrite H11.
+        destruct (GV2val (los, nts) gv); eauto; destruct v0; eauto.
+    destruct Hinsn_ext as [gv2 Hinsn_ext].
+    exists 
+         {|
+         CurSystem := s;
+         CurTargetData := (los, nts);
+         CurProducts := ps;
+         ECS := {|
+                CurFunction := f;
+                CurBB := block_intro l1 ps1
+                           (cs1 ++ insn_ext i0 e t v t0 :: cs) tmn;
+                CurCmds := cs;
+                Terminator := tmn;
+                Locals := (updateAddAL _ lc i0 gv2);
+                Allocas := als |} :: ecs;
+         Globals := gl;
+         FunTable := fs;
+         Mem := M |}.
+     exists trace_nil. eauto.
+*)
+  SCase "cast". 
+    left.
+    assert (exists gvs2, NDopsem.CAST (los,nts) lc gl c t v t0 = Some gvs2) 
+      as Hinsn_cast.
+      unfold NDopsem.CAST.      
+      assert (exists gv, NDopsem.getOperandValue (los, nts) v lc gl = Some gv) 
+        as J.
+        eapply getOperandValue_inCmdOps_isnt_stuck; eauto.
+          simpl; auto.
+      destruct J as [gv J].
+      rewrite J. eauto.
+      
+    destruct Hinsn_cast as [gv2 Hinsn_cast].
+    exists 
+         {|
+         NDopsem.CurSystem := s;
+         NDopsem.CurTargetData := (los, nts);
+         NDopsem.CurProducts := ps;
+         NDopsem.ECS := {|
+                NDopsem.CurFunction := f;
+                NDopsem.CurBB := block_intro l1 ps1
+                           (cs1 ++ insn_cast i0 c t v t0 :: cs) tmn;
+                NDopsem.CurCmds := cs;
+                NDopsem.Terminator := tmn;
+                NDopsem.Locals := (updateAddAL _ lc i0 gv2);
+                NDopsem.Allocas := als |} :: ecs;
+         NDopsem.Globals := gl;
+         NDopsem.FunTable := fs;
+         NDopsem.Mem := M |}.
+     exists trace_nil. eauto.
+
+  SCase "icmp". admit.
+(*
+    left.
+    assert (exists gv2, ICMP (los,nts) lc gl c t v v0 = Some gv2) 
+      as Hinsn_icmp.
+      unfold ICMP.      
+      assert (exists gv, getOperandValue (los, nts) v lc gl = Some gv) as J.
+        eapply getOperandValue_inCmdOps_isnt_stuck; eauto.
+          simpl; auto.
+      destruct J as [gv J].
+      rewrite J.
+      assert (exists gv, getOperandValue (los, nts) v0 lc gl = Some gv) as J0.
+        eapply getOperandValue_inCmdOps_isnt_stuck; eauto.
+          simpl; auto.
+      destruct J0 as [gv0 J0].
+      rewrite J0.
+      unfold micmp.
+      inv Hwfc. 
+      unfold isPointerTyp in H11. unfold is_true in H11.
+      unfold micmp_int.
+      destruct H11 as [H11 | H11].
+        destruct t; try solve [simpl in H11; contradict H11; auto].
+        destruct (GV2val (los,nts) gv); eauto.
+        destruct v1; eauto.
+        destruct (GV2val (los,nts) gv0); eauto.
+        destruct v1; eauto.
+        destruct c; eauto.
+
+        destruct t; try solve [simpl in H11; contradict H11; auto]. eauto.
+(*      destruct (mptrtoint (los, nts) M gv Size.ThirtyTwo); eauto.
+        destruct (mptrtoint (los, nts) M gv0 Size.ThirtyTwo); eauto.
+        destruct (GV2val (los, nts) g); eauto.
+        destruct v1; eauto.
+        destruct (GV2val (los, nts) g0); eauto.
+        destruct v1; eauto.
+        destruct c; eauto. *)
+    destruct Hinsn_icmp as [gv2 Hinsn_icmp].
+    exists 
+         {|
+         CurSystem := s;
+         CurTargetData := (los, nts);
+         CurProducts := ps;
+         ECS := {|
+                CurFunction := f;
+                CurBB := block_intro l1 ps1
+                           (cs1 ++ insn_icmp i0 c t v v0 :: cs) tmn;
+                CurCmds := cs;
+                Terminator := tmn;
+                Locals := (updateAddAL _ lc i0 gv2);
+                Allocas := als |} :: ecs;
+         Globals := gl;
+         FunTable := fs;
+         Mem := M |}.
+     exists trace_nil. eauto.
+*)
+  SCase "fcmp". admit.
+(*
+    left.
+    assert (exists gv2, FCMP (los,nts) lc gl f0 f1 v v0 = Some gv2) 
+      as Hinsn_fcmp.
+      unfold FCMP.      
+      assert (exists gv, getOperandValue (los, nts) v lc gl = Some gv) as J.
+        eapply getOperandValue_inCmdOps_isnt_stuck; eauto.
+          simpl; auto.
+      destruct J as [gv J].
+      rewrite J.
+      assert (exists gv, getOperandValue (los, nts) v0 lc gl = Some gv) as J0.
+        eapply getOperandValue_inCmdOps_isnt_stuck; eauto.
+          simpl; auto.
+      destruct J0 as [gv0 J0].
+      rewrite J0.
+      unfold mfcmp.
+      inv Hwfc. 
+      destruct (GV2val (los, nts) gv); eauto.
+      destruct v1; eauto.
+      destruct (GV2val (los, nts) gv0); eauto.
+      destruct v1; eauto.
+      apply wf_value__wf_typ in H10.
+      destruct H10 as [J1 J2].
+      destruct f1; try solve [eauto | inversion J1].
+        destruct f0; try solve [eauto | inversion H8].
+        destruct f0; try solve [eauto | inversion H8].
+    destruct Hinsn_fcmp as [gv2 Hinsn_fcmp].
+    exists 
+         {|
+         CurSystem := s;
+         CurTargetData := (los, nts);
+         CurProducts := ps;
+         ECS := {|
+                CurFunction := f;
+                CurBB := block_intro l1 ps1
+                           (cs1 ++ insn_fcmp i0 f0 f1 v v0 :: cs) tmn;
+                CurCmds := cs;
+                Terminator := tmn;
+                Locals := (updateAddAL _ lc i0 gv2);
+                Allocas := als |} :: ecs;
+         Globals := gl;
+         FunTable := fs;
+         Mem := M |}.
+     exists trace_nil. eauto.
+*)
+  SCase "select". admit.
+(*
+    assert (exists gv, getOperandValue (los, nts) v lc gl = Some gv) as J.
+      eapply getOperandValue_inCmdOps_isnt_stuck; eauto.
+        simpl; auto.
+    destruct J as [gv J].
+    assert (exists gv0, getOperandValue (los, nts) v0 lc gl = Some gv0) as J0.
+      eapply getOperandValue_inCmdOps_isnt_stuck; eauto.
+        simpl; auto.
+    destruct J0 as [gv0 J0].
+    assert (exists gv1, getOperandValue (los, nts) v1 lc gl = Some gv1) as J1.
+      eapply getOperandValue_inCmdOps_isnt_stuck; eauto.
+        simpl; auto.
+    destruct J1 as [gv1 J1].
+    left.
+    exists 
+         {|
+         CurSystem := s;
+         CurTargetData := (los, nts);
+         CurProducts := ps;
+         ECS := {|
+                CurFunction := f;
+                CurBB := block_intro l1 ps1
+                           (cs1 ++ insn_select i0 v t v0 v1 :: cs) tmn;
+                CurCmds := cs;
+                Terminator := tmn;
+                Locals := (if isGVZero (los, nts) gv 
+                           then updateAddAL _ lc i0 gv1 
+                           else updateAddAL _ lc i0 gv0);
+                Allocas := als |} :: ecs;
+         Globals := gl;
+         FunTable := fs;
+         Mem := M |}.
+     exists trace_nil. eauto.
+*)
+  SCase "call". 
+    assert (exists gvs, NDopsem.params2GVs (los, nts) p lc gl = Some gvs) as G.
+      eapply params2GVs_isnt_stuck; eauto. 
+        exists nil. auto.
+    destruct G as [gvs G].
+    assert (exists fptrs, NDopsem.getOperandValue (los, nts) v lc gl = 
+      Some fptrs) as J'.
+      eapply getOperandValue_inCmdOps_isnt_stuck; eauto.
+        simpl; auto.
+    destruct J' as [fptrs J'].
+    destruct (classic (exists fptr, exists f', fptr @ fptrs /\ 
+                      lookupFdefViaPtr ps fs fptr = Some f')) as 
+      [[fptr [f' [Hgvin HeqHlk]]] | Hnex].
+    SSCase "internal call".
+    destruct f' as [[fa rt fid la va] lb].
+    assert (J:=HeqHlk).
+    apply lookupFdefViaPtr_inversion in J; auto.
+    destruct J as [fn [Hlkft J]].
+    apply lookupFdefViaIDFromProducts_inv in J; auto.
+    eapply wf_system__wf_fdef in J; eauto.
+    inv J. destruct block5 as [l5 ps5 cs5 tmn5].
+    left.
+    exists 
+         {|
+         NDopsem.CurSystem := s;
+         NDopsem.CurTargetData := (los, nts);
+         NDopsem.CurProducts := ps;
+         NDopsem.ECS :=(NDopsem.mkEC 
+                       (fdef_intro (fheader_intro fa rt fid la va) lb) 
+                       (block_intro l5 ps5 cs5 tmn5) cs5 tmn5 
+                       (NDopsem.initLocals la gvs) 
+                       nil)::
+               {|
+                NDopsem.CurFunction := f;
+                NDopsem.CurBB := block_intro l1 ps1
+                           (cs1 ++ insn_call i0 n c t v p :: cs) tmn;
+                NDopsem.CurCmds := insn_call i0 n c t v p :: cs;
+                NDopsem.Terminator := tmn;
+                NDopsem.Locals := lc;
+                NDopsem.Allocas := als |} :: ecs;
+         NDopsem.Globals := gl;
+         NDopsem.FunTable := fs;
+         NDopsem.Mem := M |}.
+    exists trace_nil.
+    eauto.     
+(*
+    remember (lookupExFdecViaGV (los, nts) ps gl lc fs v) as Helk. 
+    destruct Helk as [f' |].
+    SSCase "external call".
+    destruct f' as [[fa rt fid la va]].
+    remember (callExternalFunction M fid gvs) as R.
+      destruct R as [[oresult Mem']|].
+      remember (exCallUpdateLocals n i0 oresult lc) as R'.
+      destruct R' as [lc' |].
+        left.
+        exists 
+         {|
+         CurSystem := s;
+         CurTargetData := (los, nts);
+         CurProducts := ps;
+         ECS :={|
+                CurFunction := f;
+                CurBB := block_intro l1 ps1
+                           (cs1 ++ insn_call i0 n c t v p :: cs) tmn;
+                CurCmds := cs;
+                Terminator := tmn;
+                Locals := lc';
+                Allocas := als |} :: ecs;
+         Globals := gl;
+         FunTable := fs;
+         Mem := Mem' |}.
+        exists trace_nil.
+        eauto.     
+
+        right.
+        unfold undefined_state.
+        right. rewrite <- HeqHlk. rewrite <- HeqHelk. rewrite G. 
+        rewrite <- HeqR0.
+        rewrite <- HeqR'. undefbehave.
+
+      right.
+      unfold undefined_state.
+      right. rewrite <- HeqHlk. rewrite <- HeqHelk. rewrite G.
+      rewrite <- HeqR0. undefbehave.
+*)
+    SSCase "stuck".
+      right.
+      unfold undefined_state.
+      right. rewrite J'. undefbehave.
+Qed.
+
+
+(*****************************)
+(*
+*** Local Variables: ***
+*** coq-prog-name: "coqtop" ***
+*** coq-prog-args: ("-emacs-U" "-I" "~/SVN/sol/vol/src/ssa/monads" "-I" "~/SVN/sol/vol/src/ssa/ott" "-I" "~/SVN/sol/vol/src/ssa/compcert" "-I" "~/SVN/sol/theory/metatheory_8.3" "-I" "~/SVN/sol/vol/src/TV") ***
+*** End: ***
+ *)
